WIP Simple form proof

coq/SimpleForm.v
@@ -1,8 +1,9 @@
 (*! Proving | Transformation of a schedule into a proof-friendly form !*)
 Require Import Coq.Numbers.DecimalString Coq.Program.Equality Coq.Strings.Ascii.
-Require Import Koika.BitsToLists Koika.Primitives Koika.Syntax.
+Require Import Koika.Primitives Koika.Syntax.
 From RecordUpdate Require Import RecordSet.
 Import RecordSetNotations.
+Require Import UntypedSemantics Koika.BitsToLists.
 
 (* When reasoning about a Koîka schedule, a lot of tedious implicit mechanisms
    have to be considered explicitly (rules merging, cancellation, ...).
@@ -26,15 +27,17 @@ Section SimpleForm.
   Context {pos_t reg_t ext_fn_t rule_name_t: Type}.
   Context {reg_t_eq_dec: EqDec reg_t}.
   Context {ext_fn_t_eq_dec: EqDec ext_fn_t}.
-  Definition uact := uaction pos_t string string reg_t ext_fn_t.
+  Definition uact := @daction pos_t string string reg_t ext_fn_t.
   Definition schedule := scheduler pos_t rule_name_t.
 
-  Definition const_nil :=
-    @UConst pos_t string string reg_t ext_fn_t (bits_t 0) (Bits.of_nat 0 0).
-  Definition const_true :=
-    @UConst pos_t string string reg_t ext_fn_t (bits_t 1) (Bits.of_nat 1 1).
+  Definition const_nil {reg_t ext_fn_t} :=
+    @DConst pos_t string string reg_t ext_fn_t (bits_t 0) (Bits.of_nat 0 0).
+  Definition const_true {reg_t ext_fn_t} :=
+    @DConst pos_t string string reg_t ext_fn_t (bits_t 1) (Bits.of_nat 1 1).
+  Definition const_false {reg_t ext_fn_t} :=
+    @DConst pos_t string string reg_t ext_fn_t (bits_t 1) (Bits.of_nat 1 0).
 
-  (* * Simple form and related structures *)
+  (* Simple form and related structures *)
   Definition cond_log := list (reg_t * uact).
   Record write_info := mkWriteInfo { wcond: uact; wval: uact }.
   Definition write_log := list (reg_t * list (write_info)).
@@ -86,123 +89,88 @@ Section SimpleForm.
   (* TODO name collisions with previously standing variables can't possibly
        happen anymore (we treat everything in order). This makes it easier to
        give informative names to our variables. *)
-  Inductive binding_type :=
-  | ctxb | letb | extcb | wcondb | fcond_ncb | fcond_cb | ivalb | fvalb.
-  Record next_ids := mkNextIds { ctx_id: nat; let_id: nat; extc_id: nat }.
-  Instance etaNextIds : Settable _ :=
-    settable! mkNextIds < ctx_id; let_id; extc_id >.
 
-  Definition initial_ids : next_ids :=
-    {| ctx_id := 0; let_id := 0; extc_id := 0 |}.
+  Definition generate_binding_name (n: nat) : string :=
+    String.append "internal_var_" (NilEmpty.string_of_uint (Init.Nat.to_uint n)).
 
-  Definition get_prefix (b: binding_type) : string :=
-    match b with
-    | ctxb => "ctx_" | letb => "let_" | extcb => "extc_" | wcondb => "wcond_"
-    | fcond_ncb => "fcond_nc_" | fcond_cb => "fcond_c_" | ivalb => "ival_"
-    | fvalb => "fval_"
-    end.
-
-  Definition generate_binding_name (b: binding_type) (n: nat) : string :=
-    String.append (get_prefix b) (NilEmpty.string_of_uint (Init.Nat.to_uint n)).
+  Definition uor (x y: uact) := DBinop (PrimUntyped.UBits2 PrimUntyped.UOr) x y.
+  Definition uand (x y: uact) := DBinop (PrimUntyped.UBits2 PrimUntyped.UAnd) x y.
+  Definition unot (x: uact) := DUnop (PrimUntyped.UBits1 PrimUntyped.UNot) x.
 
   (* * rule_information extraction *)
   (* ** Addition of a new action into an existing rule_information *)
   (* *** Merger of failure conditions *)
   Definition or_conds (conds: list uact) :=
-    fold_left
-      (fun acc c =>
-        match acc with
-        | None => Some c
-        | Some x => Some (UBinop (PrimUntyped.UBits2 PrimUntyped.UOr) c x)
-        end)
-      conds None.
+    fold_left uor conds const_false.
 
-  Definition merge_failures (f1 f2: option uact) : option uact :=
-    match f1, f2 with
-    | None, None => None
-    | Some x, None => Some x
-    | None, Some x => Some x
-    | Some x, Some y => Some (UBinop (PrimUntyped.UBits2 PrimUntyped.UOr) x y)
-    end.
+  Definition merge_failures (f1 f2: uact) : uact := uor f1 f2.
 
   Definition build_uif (cond ua1 ua2: option uact) : option uact :=
     (* We know that the original if being valid implies that cond != None and
        ua1 = Some x iff. ua2 = Some y *)
     match cond, ua1, ua2 with
-    | Some c, Some x, Some y => Some (UIf c x y)
+    | Some c, Some x, Some y => Some (DIf c x y)
     | _, _, _ => None
+    end.
+
+  Fixpoint filter_map {A B: Type} (f: A -> option B) (l: list A) : list B :=
+    match l with
+      [] => []
+    | x::r =>
+        match f x with
+        | None => filter_map f r
+        | Some b => b::filter_map f r
+        end
     end.
 
   (* *** Merger of actions *)
   (* Remove Nones from list, turn rest from (Some x) to x. *)
   Definition list_options_to_list (l: list (option uact)) : list uact :=
-    map
-      (fun i =>
-        match i with
-        | Some x => x
-        | None => const_nil (* Unreachable *)
-        end)
-      (filter (fun i => match i with None => false | Some _ => true end) l).
+    filter_map id l.
 
-  Definition merge_conds (wl: option (list write_info)) : option uact :=
-    match wl with
-    | None => None
-    | Some l => or_conds (map wcond l)
-    end.
+  Definition merge_conds (wl: (* option *) (list write_info)) : (* option  *)uact :=
+    (* match wl with *)
+    (* | None => None *)
+    (* | Some l =>  *)or_conds (map wcond wl)
+    (* end *).
 
-  Definition merge_failures_list (action_cond: uact) (conds: list uact) :=
-    match or_conds conds with
-    | None => None
-    | Some x =>
-      Some (UBinop (PrimUntyped.UBits2 PrimUntyped.UAnd) action_cond x)
-    end.
+  Definition merge_failures_list (action_cond: uact) (conds: list uact)
+    : (* option *) uact :=
+    uand action_cond (or_conds conds).
 
   Definition add_read0 (rir: rule_information_raw) (grd: uact) (reg: reg_t)
-  (* Returns modified rir, failure conditions *)
-  : rule_information_raw * option uact := (
+  (* Returns modified rir *)
+    : rule_information_raw :=
+    let new_grd :=
       match list_assoc (rir_read0s rir) reg with
-      | None =>
-        rir <| rir_read0s := list_assoc_set (rir_read0s rir) reg grd |>
-      | Some cond' =>
-        rir <| rir_read0s :=
-          list_assoc_set (rir_read0s rir) reg
-            (UBinop (PrimUntyped.UBits2 PrimUntyped.UOr) cond' grd) |>
-      end,
-      merge_failures_list grd (
-        list_options_to_list
-          [option_map fst (list_assoc (rir_write0s rir) reg);
-           option_map fst (list_assoc (rir_write1s rir) reg)])).
+      | None => grd
+      | Some cond' => uor cond' grd
+      end in
+    rir <| rir_read0s := list_assoc_set (rir_read0s rir) reg new_grd |>.
 
   Definition add_read1 (rir: rule_information_raw) (grd: uact) (reg: reg_t)
-  (* Returns modified rule_information_raw, failure conditions *)
-  : rule_information_raw * option uact := (
-    match list_assoc (rir_read1s rir) reg with
-    | None =>
-      rir <| rir_read1s := list_assoc_set (rir_read1s rir) reg grd |>
-    | Some cond' =>
-      rir <| rir_read1s :=
-        list_assoc_set (rir_read1s rir) reg
-          (UBinop (PrimUntyped.UBits2 PrimUntyped.UOr) cond' grd) |>
-    end,
-    merge_failures_list grd
-      (list_options_to_list [option_map fst (list_assoc (rir_write1s rir) reg)])
-  ).
+  (* Returns modified rule_information_raw *)
+    : rule_information_raw :=
+    let new_grd :=
+      match list_assoc (rir_read1s rir) reg with
+      | None => grd
+      | Some cond' => uor cond' grd
+      end in
+    rir <| rir_read1s := list_assoc_set (rir_read1s rir) reg new_grd |>.
 
    Definition add_write0
     (rir: rule_information_raw) (grd: uact) (reg: reg_t) (val: uact)
   (* Returns modified rule_information_raw, failure conditions *)
-  : rule_information_raw * option uact := (
-    match list_assoc (rir_write0s rir) reg with
-    | None =>
-      rir <| rir_write0s :=
-        list_assoc_set (rir_write0s rir) reg
-          (grd, [{| wcond := grd; wval := val |}]) |>
-    | Some c =>
-      rir <| rir_write0s :=
-        list_assoc_set (rir_write0s rir) reg
-          (UBinop (PrimUntyped.UBits2 PrimUntyped.UOr) (fst c) grd,
-           (snd c)++[{| wcond := grd; wval := val |}]) |>
-    end,
+     : rule_information_raw * uact :=
+     let (new_grd, new_wi) :=
+       match list_assoc (rir_write0s rir) reg with
+       | None => (grd, [{| wcond := grd; wval := val |}])
+       | Some c =>
+           (uor (fst c) grd,
+             (snd c)++[{| wcond := grd; wval := val |}])
+       end in
+     (rir <| rir_write0s :=
+        list_assoc_set (rir_write0s rir) reg (new_grd, new_wi) |>,
     merge_failures_list
       grd
       (list_options_to_list ([
@@ -213,18 +181,16 @@ Section SimpleForm.
   Definition add_write1
     (rir: rule_information_raw) (grd: uact) (reg: reg_t) (val: uact)
   (* Returns modified rule_information_raw, failure conditions *)
-  : rule_information_raw * option uact := (
-    match list_assoc (rir_write1s rir) reg with
-    | None =>
-      rir <| rir_write1s :=
-        list_assoc_set (rir_write1s rir) reg
-          (grd, [{| wcond := grd; wval := val |}]) |>
-    | Some c =>
-      rir <| rir_write1s :=
-        list_assoc_set (rir_write1s rir) reg
-          (UBinop (PrimUntyped.UBits2 PrimUntyped.UOr) (fst c) grd,
-           ((snd c)++[{| wcond := grd; wval := val |}])) |>
-    end,
+    : rule_information_raw * uact :=
+    let (new_grd, new_wi) :=
+       match list_assoc (rir_write1s rir) reg with
+       | None => (grd, [{| wcond := grd; wval := val |}])
+       | Some c =>
+           (uor (fst c) grd,
+             (snd c)++[{| wcond := grd; wval := val |}])
+       end in
+     (rir <| rir_write1s :=
+        list_assoc_set (rir_write1s rir) reg (new_grd, new_wi) |>,
     merge_failures_list grd (list_options_to_list [
       option_map fst (list_assoc (rir_write1s rir) reg)])).
 
@@ -237,238 +203,1814 @@ Section SimpleForm.
     |>.
 
   (* ** Extraction of actions from rule *)
-  Definition reduce (ua: option uact) : uact :=
+    Definition reduce (ua: option (uact)) : uact :=
     match ua with
     | None => const_nil
     | Some x => x
     end.
+  
+  Definition merge_branches
+             (vm_tb vm_fb: list (string*string))
+             (vvs: list (string * uact))
+             (nid: nat)
+             (cond_name: string) :=
+    fold_left
+      (fun '(acc, vv', let_id) '((str, n1), (_, n2)) =>
+         if String.eqb n1 n2
+         then ((str, n1)::acc, vv', let_id)
+         else
+           let name := generate_binding_name let_id in
+           (
+             (str, name)::acc,
+             vv'++[(name, DIf (DVar cond_name) (DVar n1) (DVar n2))],
+             S let_id)
+      )
+      (combine vm_tb vm_fb) ([], vvs, nid).
+
+  Fixpoint merge_branches'
+           (vm_tb vm_fb: list (string*string))
+           (vvs: list (string * uact))
+           (nid: nat)
+           (cond_name: string) :=
+    match vm_tb, vm_fb with
+    | (str, n1)::vm_tb, (_, n2)::vm_fb =>
+        let '(acc, vv', let_id) := merge_branches' vm_tb vm_fb vvs nid cond_name in
+        if String.eqb n1 n2
+        then ((str, n1)::acc, vv', let_id)
+        else let name := generate_binding_name let_id in
+             (
+               (str, name)::acc,
+               vv'++[(name, DIf (DVar cond_name) (DVar n1) (DVar n2))],
+               S let_id)
+    | _, _ => ([], vvs, nid)
+    end.
+
+  Lemma merge_branches_ok:
+    forall vm_tb vm_fb vvs nid cond_name,
+      List.length vm_tb = List.length vm_fb ->
+      merge_branches (rev vm_tb) (rev vm_fb) vvs nid cond_name =
+        merge_branches' vm_tb vm_fb vvs nid cond_name.
+  Proof.
+    induction vm_tb; simpl; intros; eauto.
+    repeat destr. simpl. unfold merge_branches. rewrite combine_nil. simpl. auto.
+    simpl.
+    unfold merge_branches in *. rewrite combine_app. rewrite fold_left_app.
+    simpl. destr. rewrite IHvm_tb in Heqp3.
+    rewrite Heqp1 in Heqp3. inv Heqp3. rewrite Heqb. reflexivity.
+    simpl in H; congruence.
+    simpl in H.
+    rewrite ! List.rev_length. congruence. reflexivity.
+    simpl in H. inv H.
+    simpl. unfold merge_branches. simpl.
+    unfold merge_branches in *. rewrite combine_app. rewrite fold_left_app.
+    simpl. destr. rewrite IHvm_tb in Heqp.
+    rewrite Heqp1 in Heqp. inv Heqp. rewrite Heqb. reflexivity.
+    auto.
+    rewrite ! List.rev_length. auto. reflexivity.
+  Qed.
+
+  Definition gria_list
+             (args: list uact)
+             (env: list (string * string))
+             vvs
+             (rir: rule_information_raw)
+             (nid: nat)
+             (guard: uact)
+             (rec: uact -> list (string * string) -> list(string * uact) -> uact -> rule_information_raw -> nat -> (option uact * list (string * string) * list (string * uact) * uact * rule_information_raw * nat ))
+             names0 fail0
+    :=
+    fold_left
+      (fun '(names, vm_p, vv_p, failures_p, rir_p, nid) a =>
+         let '(val_c, vm_c, vv_c, failure_c, rir_c, nid) :=
+           rec a vm_p vv_p guard rir_p nid
+         in
+         let arg_bind_name :=
+           generate_binding_name nid
+         in (
+           arg_bind_name::names, vm_c,
+           list_assoc_set vv_c (arg_bind_name) (reduce val_c),
+           merge_failures failure_c failures_p, rir_c,
+           S nid))
+      args
+      (names0, env, vvs, fail0, rir, nid).
+
+
+  Definition gria_list'
+             (guard: uact)
+             (rec: uact -> list (string * string) -> list(string * uact) -> uact -> rule_information_raw -> nat -> (option uact * list (string * string) * list (string * uact) * uact * rule_information_raw * nat ))
+    :=
+    fix gria_list'
+        (args: list uact)
+        (env: list (string * string))
+        (vvs: list (string * uact))
+        (rir: rule_information_raw)
+        (nid: nat)
+        names0
+        fail0
+      : list string * list (string * string) * list (string * uact) * uact * rule_information_raw * nat
+      :=
+      match args with
+        [] => (names0, env, vvs, fail0, rir, nid)
+      | a::args =>
+          let '(vc, vms, vvs, failure, rir, nid) :=
+            rec a env vvs guard rir nid in
+          let arg_bind_name := generate_binding_name nid in
+          gria_list' args vms
+                   (list_assoc_set vvs arg_bind_name (reduce vc))
+                   rir (S nid) (arg_bind_name :: names0) (merge_failures failure fail0)
+      end.
+
+  Lemma gria_list_ok:
+    forall args env vvs rir nid guard rec names0 fail0,
+      gria_list args env vvs rir nid guard rec names0 fail0 =
+        gria_list' guard rec args env vvs rir nid names0 fail0.
+  Proof.
+    induction args; simpl; intros; eauto.
+    unfold gria_list in *. simpl.
+    repeat destr. subst.
+    rewrite IHargs. auto.
+  Qed.
 
   (* This function extracts the actions for a given rule. It also returns the
      updated next_ids structure. *)
   Fixpoint get_rule_information_aux
-    (* No need to pass failures as these impact the whole rule - taking note of
+           (* No need to pass failures as these impact the whole rule - taking note of
        all of them and factoring the conditions in is enough. Conflicts between
        different actions are also dealt with here. *)
-    (* TODO improve guards management *)
-    (* TODO guard could be option string instead *)
-    (ua: uact) (env: list (string * string)) (guard: uact)
-    (rir: rule_information_raw) (nid: next_ids)
+           (* TODO improve guards management *)
+           (* TODO guard could be option string instead *)
+           (ua: uact) (env: list (string * string))
+           (vvs: list (string * uact))
+           (guard: uact)
+           (rir: rule_information_raw) (nid: nat)
     (* Returns value, env, var_values, failure condition, rule_information_raw,
        next_ids *)
-  : option uact * list (string * string) * (list (string * uact))
-    * (option uact) * rule_information_raw * next_ids
+    : option (uact)
+      * list (string * string)
+      * (list (string * uact))
+      * (uact) * rule_information_raw * nat
     (* TODO remove redundancies with rule_information_raw (failure_cond,
          var_values) *)
-  :=
+    :=
     match ua with
-    | UBind var val body =>
-      let '(ret_val, vm_val, vv_val, failures_val, rir_val, nid_val) :=
-        get_rule_information_aux val env guard rir nid
-      in
-      let name := generate_binding_name letb (S (let_id nid_val)) in
-      let '(ret_body, vm_body, vv_body, failures_body, rir_body, nid_body) :=
-        get_rule_information_aux
-          body ((var, name)::env) guard rir_val
-          (nid_val <| let_id := S (let_id nid_val) |>)
-      in (
-        ret_body, skipn 1 vm_body (* var's binding goes out of scope *),
-        vv_val++[(name, reduce ret_val)]++vv_body,
-        merge_failures failures_val failures_body, rir_body, nid_body)
-    | UAssign var val =>
-      let '(ret_val, vm_val, vv_val, failures_val, rir_val, nid_val) :=
-        get_rule_information_aux val env guard rir nid
-      in
-      let name := generate_binding_name letb (S (let_id nid_val)) in
-      (None, list_assoc_set vm_val var name, vv_val++[(name, reduce ret_val)],
-       failures_val, rir_val, nid_val <| let_id := S (let_id nid_val) |>
-      )
-    | UVar var =>
-      match list_assoc env var with
-      | Some x => (Some (UVar x), env, [], None, rir, nid)
-      | None => (* Unreachable assuming rule valid *)
-        (Some (UVar "ERROR"), env, [], None, rir, nid)
-      end
-    | USeq a1 a2 =>
-      let '(_, vm_a1, vv_a1, failures_a1, rir_a1, nid_a1) :=
-        get_rule_information_aux a1 env guard rir nid
-      in
-      let '(ret_a2, vm_a2, vv_a2, failures_a2, rir_a2, nid_a2) :=
-        get_rule_information_aux a2 vm_a1 guard rir_a1 nid_a1
-      in
-      (ret_a2, vm_a2, vv_a1++vv_a2, merge_failures failures_a1 failures_a2,
-       rir_a2, nid_a2)
-    | UIf cond tb fb =>
-      let '(ret_cond, vm_cond, vv_cond, failures_cond, rir_cond, nid_cond) :=
-        get_rule_information_aux cond env guard rir nid
-      in
-      let cond_name := generate_binding_name ctxb (ctx_id nid_cond + 1) in
-      let guard_tb_name := generate_binding_name ctxb (ctx_id nid_cond + 2) in
-      let guard_fb_name := generate_binding_name ctxb (ctx_id nid_cond + 3) in
-      let guard_tb :=
-        UBinop (PrimUntyped.UBits2 PrimUntyped.UAnd) guard (UVar cond_name)
-      in
-      let guard_fb :=
-        UBinop (PrimUntyped.UBits2 PrimUntyped.UAnd)
-          guard (UUnop (PrimUntyped.UBits1 PrimUntyped.UNot) (UVar cond_name))
-      in
-      let '(ret_tb, vm_tb, vv_tb, failures_tb, rir_tb, nid_tb) :=
-        get_rule_information_aux tb vm_cond (UVar guard_tb_name) rir_cond
-        (nid_cond <| ctx_id := (ctx_id nid_cond + 3) |>)
-      in
-      let '(ret_fb, vm_fb, vv_fb, failures_fb, rir_fb, nid_fb) :=
-        (* We use rir_tb here even though we know that none of the actions added
+    | DBind var val body =>
+        let '(ret_val, vm_val, vv_val, failures_val, rir_val, nid) :=
+          get_rule_information_aux val env vvs guard rir nid
+        in
+        let name := generate_binding_name nid in
+        let '(ret_body, vm_body, vv_body, failures_body, rir_body, nid) :=
+          get_rule_information_aux
+            body
+            ((var, name)::env)
+            (list_assoc_set vv_val name (reduce ret_val))
+            guard
+            rir_val
+            (S nid)
+        in (
+          ret_body, skipn 1 vm_body (* var's binding goes out of scope *),
+          vv_body,
+          merge_failures failures_val failures_body, rir_body, nid)
+    | DAssign var val =>
+        let '(ret_val, vm_val, vv_val, failures_val, rir_val, nid) :=
+          get_rule_information_aux val env vvs guard rir nid
+        in
+        let name := generate_binding_name nid in
+        (None,
+          list_assoc_set vm_val var name,
+          list_assoc_set vv_val name (reduce ret_val),
+          failures_val, rir_val, S nid
+        )
+    | DVar var =>
+        match list_assoc env var with
+        | Some x => (Some (DVar x), env, vvs, const_false, rir, nid)
+        | None => (* Unreachable assuming rule valid *)
+            (None, env, vvs, const_true, rir, nid)
+        end
+    | DSeq a1 a2 =>
+        let '(_, vm_a1, vv_a1, failures_a1, rir_a1, nid_a1) :=
+          get_rule_information_aux a1 env vvs guard rir nid
+        in
+        let '(ret_a2, vm_a2, vv_a2, failures_a2, rir_a2, nid_a2) :=
+          get_rule_information_aux a2 vm_a1 vv_a1 guard rir_a1 nid_a1
+        in
+        (ret_a2, vm_a2, vv_a2, merge_failures failures_a1 failures_a2,
+          rir_a2, nid_a2)
+    | DIf cond tb fb =>
+        let '(ret_cond, vm_cond, vv_cond, failures_cond, rir_cond, nid) :=
+          get_rule_information_aux cond env vvs guard rir nid
+        in
+        let cond_name := generate_binding_name nid in
+        let guard_tb_name := generate_binding_name (nid + 1) in
+        let guard_fb_name := generate_binding_name (nid + 2) in
+        let guard_tb := uand guard (DVar cond_name) in
+        let guard_fb := uand guard (unot (DVar cond_name)) in
+        let vv_cond := list_assoc_set vv_cond cond_name (reduce ret_cond) in
+        let vv_cond := list_assoc_set vv_cond guard_tb_name guard_tb in
+        let vv_cond := list_assoc_set vv_cond guard_fb_name guard_fb in
+        let '(ret_tb, vm_tb, vv_tb, failures_tb, rir_tb, nid) :=
+          get_rule_information_aux tb vm_cond vv_cond (DVar guard_tb_name) rir_cond
+                                   (nid + 3)
+        in
+        let '(ret_fb, vm_fb, vv_fb, failures_fb, rir_fb, nid) :=
+          (* We use rir_tb here even though we know that none of the actions added
            by the other branch can impact those from this branch (they are
            mutually exclusive). This way, we don't have to deal with
            rule_information_raw merging. However, this also means that the
            failure condition will contain some redundancy. *)
-        get_rule_information_aux fb vm_cond (UVar guard_fb_name) rir_tb nid_tb
-      in
-      (* Merge var maps: if vm_tb and vm_fb disagree for some variable, generate
+          get_rule_information_aux fb vm_cond vv_tb (DVar guard_fb_name) rir_tb nid
+        in
+        (* Merge var maps: if vm_tb and vm_fb disagree for some variable, generate
          a new variable reflecting the condition and update the variables map.
-       *)
-      let '(vm_merge, vv_merge, let_id_merge) :=
-        fold_left
-          (fun '(acc, vv', let_id) '((str, n1), (_, n2)) =>
-            if String.eqb n1 n2 then ((str, n1)::acc, vv', let_id)
-            else
-              let name := generate_binding_name letb (S let_id) in (
-                (str, name)::acc,
-                vv'++[(name, UIf (UVar cond_name) (UVar n1) (UVar n2))],
-                S let_id))
-          (combine vm_tb vm_fb) ([], [], let_id nid_fb)
-      in
-      (build_uif ret_cond ret_tb ret_fb, vm_merge,
-       vv_cond++[
-         (cond_name, reduce ret_cond); (guard_tb_name, guard_tb);
-         (guard_fb_name, guard_fb)
-       ]++vv_tb++vv_fb++vv_merge,
-       (* Merging the failure conditions: looks complex because of the option
+         *)
+        let '(vm_merge, vv_merge, nid) := merge_branches' vm_tb vm_fb vv_fb nid cond_name in
+        (build_uif ret_cond ret_tb ret_fb,
+          vm_merge,
+          vv_merge,
+          (* Merging the failure conditions: looks complex because of the option
           types but really not that tricky. *)
-       match ret_cond with
-       | None => None (* Unreachable assuming a well-formed rule *)
-       | Some x =>
-         merge_failures
-           failures_cond
-           (merge_failures
-             (option_map
-               (fun y => UBinop (PrimUntyped.UBits2 PrimUntyped.UAnd) x y)
-               failures_tb)
-             (option_map
-               (fun y =>
-                 (UBinop (PrimUntyped.UBits2 PrimUntyped.UAnd)
-                   (UUnop (PrimUntyped.UBits1 PrimUntyped.UNot) x) y))
-               failures_fb))
-        end,
-        rir_fb, nid_fb <| let_id := let_id_merge |>)
-    | UUnop ufn a =>
-      let '(ret_a, vm_a, vv_a, failures_a, rir_a, nid_a) :=
-        get_rule_information_aux a env guard rir nid
-      in
-      (Some (UUnop ufn (reduce ret_a)), vm_a, vv_a, failures_a, rir_a, nid_a)
-    | UBinop ufn a1 a2 =>
-      let '(ret_a1, vm_a1, vv_a1, failures_a1, rir_a1, nid_a1) :=
-        get_rule_information_aux a1 env guard rir nid
-      in
-      let '(ret_a2, vm_a2, vv_a2, failures_a2, rir_a2, nid_a2) :=
-        get_rule_information_aux a2 vm_a1 guard rir_a1 nid_a1
-      in
-      (Some (UBinop ufn (reduce ret_a1) (reduce ret_a2)), vm_a2, vv_a1++vv_a2,
-       merge_failures failures_a1 failures_a2, rir_a2, nid_a2)
-    | UInternalCall ufn args =>
-      let '(arg_names, vm_args, vv_args, failure_args, rir_args, nid_args) := (
-        fold_left
-          (fun '(names, vm_p, vv_p, failures_p, rir_p, nid_p) a =>
-            let '(val_c, vm_c, vv_c, failure_c, rir_c, nid_c) :=
-              get_rule_information_aux a vm_p guard rir_p nid_p
-            in
-            let arg_bind_name :=
-              generate_binding_name letb (S (let_id nid_c))
-            in (
-              arg_bind_name::names, vm_c,
-              vv_p++vv_c++[(arg_bind_name, reduce val_c)],
-              merge_failures failure_c failures_p, rir_c,
-              nid_c <| let_id := S (let_id nid_c) |>))
-          args
-          ([], env, [], None, rir, nid)
-      ) in
-      let vm_tmp :=
-        combine
-          (fst (split (int_argspec ufn))) (* Names from argspec *)
-          (* We know that a value is assigned to each argument in well formed
+          match ret_cond with
+          | None => const_true (* Unreachable assuming a well-formed rule *)
+          | Some x =>
+              uor failures_cond
+                  (uor
+                     (uand x failures_tb)
+                     (uand (unot x) failures_fb)
+                  )
+          end,
+          rir_fb, nid)
+    | DUnop ufn a =>
+        let '(ret_a, vm_a, vv_a, failures_a, rir_a, nid) :=
+          get_rule_information_aux a env vvs guard rir nid
+        in
+        (Some (DUnop ufn (reduce ret_a)), vm_a, vv_a, failures_a, rir_a, nid)
+    | DBinop ufn a1 a2 =>
+        let '(ret_a1, vm_a1, vvs, failures_a1, rir_a1, nid) :=
+          get_rule_information_aux a1 env vvs guard rir nid
+        in
+        let '(ret_a2, vm_a2, vvs, failures_a2, rir_a2, nid) :=
+          get_rule_information_aux a2 vm_a1 vvs guard rir_a1 nid
+        in
+        (Some (DBinop ufn (reduce ret_a1) (reduce ret_a2)), vm_a2, vvs,
+          merge_failures failures_a1 failures_a2, rir_a2, nid)
+    | DInternalCall ufn args =>
+        let '(arg_names, vm_args, vv_args, failure_args, rir_args, nid) :=
+          gria_list' guard get_rule_information_aux args env vvs rir nid [] const_false in
+        let vm_tmp :=
+          combine
+            (fst (split (int_argspec ufn))) (* Names from argspec *)
+            (* We know that a value is assigned to each argument in well formed
              rules *)
-          arg_names
-      in
-      let '(ret_ic, _, vv_ic, failure_ic, rir_ic, nid_ic) :=
-        get_rule_information_aux (int_body ufn) vm_tmp guard rir_args nid_args
-      in
-      (* We can forget vm_tmp which contained the temporary map for use in the
+            arg_names
+        in
+        let '(ret_ic, _, vv_ic, failure_ic, rir_ic, nid) :=
+          get_rule_information_aux (int_body ufn) vm_tmp vv_args guard rir_args nid
+        in
+        (* We can forget vm_tmp which contained the temporary map for use in the
          called function. *)
-      (ret_ic, vm_args, vv_args++vv_ic, merge_failures failure_ic failure_args,
-       rir_ic, nid_ic)
-    | UAPos _ e => get_rule_information_aux e env guard rir nid
-    | URead port reg =>
-      let '(modified_rir, failure_read) :=
-        match port with
-        | P0 => add_read0 rir guard reg
-        | P1 => add_read1 rir guard reg
-        end
-      in (Some ua, env, [], failure_read, modified_rir, nid)
-    | UWrite port reg val =>
-      let '(ret_val, vm_val, vv_val, failures_val, actions_val, nid_val) :=
-        get_rule_information_aux val env guard rir nid
-      in
-      let '(rir_wr, failure_wr) :=
-        match port with
-        | P0 => add_write0 actions_val guard reg (reduce ret_val)
-        | P1 => add_write1 actions_val guard reg (reduce ret_val)
-        end
-      in
-      (None, vm_val, vv_val, merge_failures failures_val failure_wr, rir_wr,
-       nid_val)
-    | UExternalCall ufn arg =>
-      let '(ret_arg, vm_arg, vv_arg, failures_arg, actions_arg, nid_arg) :=
-        get_rule_information_aux arg env guard rir nid
-      in
-      let name := generate_binding_name extcb (S (extc_id nid_arg)) in
-      let new_rir := add_extcall rir guard ufn arg name in
-      (Some (UVar name), vm_arg, vv_arg, failures_arg, new_rir,
-       nid_arg <| extc_id := S (extc_id nid_arg) |>)
-    | UError _ => (None, env, [], Some (const_true), rir, nid)
-    | UFail _ => (None, env, [], Some (const_true), rir, nid)
-    | _ => (Some ua, env, [], None, rir, nid) (* UConst *)
+        (ret_ic, vm_args, vv_ic, merge_failures failure_ic failure_args,
+          rir_ic, nid)
+    | DAPos _ e => get_rule_information_aux e env vvs guard rir nid
+    | DRead port reg =>
+        let modified_rir :=
+          match port with
+          | P0 => add_read0 rir guard reg
+          | P1 => add_read1 rir guard reg
+          end
+        in (Some ua, env, vvs, const_false, modified_rir, nid)
+    | DWrite port reg val =>
+        let '(ret_val, vm_val, vv_val, failures_val, actions_val, nid) :=
+          get_rule_information_aux val env vvs guard rir nid
+        in
+        let '(rir_wr, failure_wr) :=
+          match port with
+          | P0 => add_write0 actions_val guard reg (reduce ret_val)
+          | P1 => add_write1 actions_val guard reg (reduce ret_val)
+          end
+        in
+        (None, vm_val, vv_val, merge_failures failures_val failure_wr, rir_wr,
+          nid)
+    | DExternalCall ufn arg =>
+        let '(ret_arg, vm_arg, vv_arg, failures_arg, actions_arg, nid) :=
+          get_rule_information_aux arg env vvs guard rir nid
+        in
+        let name := generate_binding_name nid in
+        let new_rir := add_extcall rir guard ufn (reduce ret_arg) name in
+        (Some (DVar name), vm_arg, vv_arg, failures_arg, new_rir,
+          S nid)
+    | DError _ => (None, env, vvs, const_true, rir, nid)
+    | DFail _ => (None, env, vvs, const_true, rir, nid)
+    | DConst _ => (Some ua, env, vvs, const_false, rir, nid)
     end.
 
-  Definition get_rule_information (ua: uact) (nid: next_ids)
-  : rule_information_raw * next_ids :=
+  Inductive simple_shape : uact -> Prop :=
+  | simple_shape_var v: simple_shape (DVar v)
+  | simple_shape_const tau (v: type_denote tau): simple_shape (DConst v)
+  | simple_shape_if c t f:
+    simple_shape c -> simple_shape t -> simple_shape f ->
+    simple_shape (DIf c t f)
+  | simple_shape_unop ufn a: simple_shape a -> simple_shape (DUnop ufn a)
+  | simple_shape_binop ufn a1 a2: simple_shape a1 -> simple_shape a2 -> simple_shape (DBinop ufn a1 a2)
+  | simple_shape_read prt idx: simple_shape (DRead prt idx)
+  .
+
+  Lemma get_rule_information_aux_act_shape:
+    forall (ua: uact)
+           (env: list (string * string)) (guard: uact)
+           (rir: rule_information_raw) (nid: nat)
+           v env' vvs vvs0 fail_cond rir' nid'
+           (GRIA: get_rule_information_aux ua env vvs0 guard rir nid = (Some v, env', vvs, fail_cond, rir', nid')),
+      simple_shape v.
+  Proof.
+    intros ua; pattern ua.
+    eapply daction_ind'; simpl; intros; eauto.
+    - inv GRIA.
+    - inv GRIA.
+    - repeat destr_in GRIA; inv GRIA; constructor.
+    - repeat destr_in GRIA; inv GRIA; constructor.
+    - repeat destr_in GRIA; inv GRIA; constructor.
+    - repeat destr_in GRIA; inv GRIA. eauto.
+    - repeat destr_in GRIA; inv GRIA; eauto.
+    - repeat destr_in GRIA; inv GRIA.
+      repeat destr_in H3; inv H3. constructor; eauto.
+    - repeat destr_in GRIA; inv GRIA; constructor.
+    - repeat destr_in GRIA; inv GRIA.
+    - repeat destr_in GRIA; inv GRIA. constructor. unfold reduce; destr. eauto. constructor.
+    - repeat destr_in GRIA; inv GRIA. constructor.
+      unfold reduce; destr. eauto. constructor.
+      unfold reduce; destr. eauto. constructor.
+    - repeat destr_in GRIA; inv GRIA. constructor.
+    - repeat destr_in GRIA; inv GRIA. eauto.
+  Qed.
+
+  
+  Inductive var_in_uact : uact -> string -> Prop :=
+  | var_in_uact_var v: var_in_uact (DVar v) v
+  | var_in_if_cond c t f v:
+    var_in_uact c v ->
+    var_in_uact (DIf c t f) v
+  | var_in_if_true c t f v:
+    var_in_uact f v ->
+    var_in_uact (DIf c t f) v
+  | var_in_if_false c t f v:
+    var_in_uact t v ->
+    var_in_uact (DIf c t f) v
+  | var_in_uact_unop ufn a v:
+    var_in_uact a v -> var_in_uact (DUnop ufn a) v
+  | var_in_uact_binop_1 ufn a1 a2 v:
+    var_in_uact a1 v -> var_in_uact (DBinop ufn a1 a2) v
+  | var_in_uact_binop_2 ufn a1 a2 v:
+    var_in_uact a2 v -> var_in_uact (DBinop ufn a1 a2) v.
+
+
+  Lemma list_assoc_set_key_in:
+    forall {K V: Type} {eq_dec_k: EqDec K} (l: list (K*V)) k v,
+      In k (map fst (list_assoc_set l k v)).
+  Proof.
+    induction l; simpl; intros; eauto.
+    repeat destr. subst; simpl; auto. simpl; eauto.
+  Qed.
+
+
+  Lemma list_assoc_set_key_stays_in:
+    forall {K V: Type} {eq_dec_k: EqDec K} (l: list (K*V)) k k' v,
+      In k (map fst l) ->
+      In k (map fst (list_assoc_set l k' v)).
+  Proof.
+    induction l; simpl; intros; eauto.
+    repeat destr. subst; simpl; auto. simpl in *; eauto.
+    destruct H; auto.
+  Qed.
+
+  Lemma list_assoc_cons:
+    forall {K V: Type} {eq_dec_k: EqDec K} (l: list (K*V)) k k' v,
+      list_assoc ((k,v)::l) k' =
+        if eq_dec k' k then Some v else list_assoc l k'.
+  Proof.
+    reflexivity.
+  Qed.
+
+  Inductive wf_uact_known_vars: list string -> uact -> Prop :=
+  | wf_uact_known_vars_error l e: wf_uact_known_vars l (DError e)
+  | wf_uact_known_vars_fail l e: wf_uact_known_vars l (DFail e)
+  | wf_uact_known_vars_var l v: In v l -> wf_uact_known_vars l (DVar v)
+  | wf_uact_known_vars_const l tau (c: type_denote tau): wf_uact_known_vars l (DConst c)
+  | wf_uact_known_vars_assign l v a:
+    wf_uact_known_vars l a ->
+    In v l ->
+    wf_uact_known_vars l (DAssign v a)
+  | wf_uact_known_vars_seq l a1 a2:
+    wf_uact_known_vars l a1 ->
+    wf_uact_known_vars l a2 ->
+    wf_uact_known_vars l (DSeq a1 a2)
+  | wf_uact_known_vars_bind l v a body :
+    wf_uact_known_vars l a ->
+    wf_uact_known_vars (v::l) body ->
+    wf_uact_known_vars l (DBind v a body)
+  | wf_uact_known_vars_if l c t f :
+    wf_uact_known_vars l c ->
+    wf_uact_known_vars l t ->
+    wf_uact_known_vars l f ->
+    wf_uact_known_vars l (DIf c t f)
+  | wf_uact_known_vars_read l p i:
+    wf_uact_known_vars l (DRead p i)
+  | wf_uact_known_vars_write l p i a:
+    wf_uact_known_vars l a ->
+    wf_uact_known_vars l (DWrite p i a)
+  | wf_uact_known_vars_unop l ufn a:
+    wf_uact_known_vars l a ->
+    wf_uact_known_vars l (DUnop ufn a)
+  | wf_uact_known_vars_binop l ufn a1 a2:
+    wf_uact_known_vars l a1 ->
+    wf_uact_known_vars l a2 ->
+    wf_uact_known_vars l (DBinop ufn a1 a2)
+  | wf_uact_known_vars_ext l ufn a:
+    wf_uact_known_vars l a ->
+    wf_uact_known_vars l (DExternalCall ufn a)
+  | wf_uact_known_vars_int l ufn a:
+    Forall (wf_uact_known_vars l) a ->
+    List.length (map fst (int_argspec ufn)) = List.length a ->
+    wf_uact_known_vars (map fst (int_argspec ufn)) (int_body ufn) ->
+    wf_uact_known_vars l (DInternalCall ufn a).
+
+  Lemma same_env_set_in:
+    forall env' env
+           (SAMEENV: Forall2 (fun x y : string * string => fst x = fst y) env env')
+           v n
+           (VARIN: In v (map fst env)) ,
+      Forall2 (fun x y : string * string => fst x = fst y) env (list_assoc_set env' v n).
+  Proof.
+    Opaque eq_dec.
+    induction env'; simpl; intros; eauto.
+    - inv SAMEENV. simpl in *; easy.
+    - inv SAMEENV. simpl in *. destr. simpl in *. subst.
+      destr.
+      + subst. simpl. constructor. reflexivity. auto.
+      + constructor. reflexivity. eapply IHenv'. eauto. destruct VARIN; congruence.
+  Qed.
+
+  Lemma same_env_trans:
+    forall {P: Type} (R: P -> P -> Prop) (Rtrans: forall x y z, R x y -> R y z -> R x z)
+           l1 l2,
+      Forall2 R l1 l2 -> forall l3, Forall2 R l2 l3 -> Forall2 R l1 l3.
+  Proof.
+    induction 2; simpl; intros; eauto. inv H1; constructor; eauto.
+  Qed.
+
+  Lemma same_env_refl:
+    forall (l: list (string * string)),
+      Forall2 (fun x y => fst x = fst y) l l.
+  Proof.
+    induction l; simpl; intros; eauto.
+  Qed.
+
+  Lemma same_env_sym:
+    forall (l1 l2: list (string * string)),
+      Forall2 (fun x y => fst x = fst y) l1 l2 ->
+      Forall2 (fun x y => fst x = fst y) l2 l1.
+  Proof.
+    induction 1; simpl; intros; eauto.
+  Qed.
+
+  Lemma same_env_same_fst:
+    forall (l1 l2: list (string * string)),
+      Forall2 (fun x y => fst x = fst y) l1 l2 ->
+      map fst l1 = map fst l2.
+  Proof.
+    induction 1; simpl; intros; eauto. congruence.
+  Qed.
+
+  Lemma merge_vms_preserve_same_env:
+    forall (l2 l4: list (string*string))
+           (F: Forall2 (fun x y => fst x = fst y) l2 l4)
+           (l3: list (string*uact)) cname n1 env' vvs n2,
+      merge_branches' l2 l4 l3 n1 cname = (env', vvs, n2) ->
+      Forall2 (fun x y => fst x = fst y) l2 env'.
+  Proof.
+    induction 1; simpl; intros; eauto.
+    - inv H. constructor.
+    - do 4 destr_in H0. apply IHF in Heqp1.
+      destr_in H0. inv H0. constructor; auto.
+      inv H0. constructor; auto.
+  Qed.
+
+
+
+  Lemma gria_list_same_env:
+    forall
+      args env
+      (F: Forall (wf_uact_known_vars (map fst env)) args)
+      (IH: Forall
+             (fun u : uact =>
+                forall (env : list (string * string)) (guard : uact)
+                       (rir : rule_information_raw) (nid : nat) 
+                       (v : option uact) (env' : list (string * string))
+                       (vvs : list (string * uact)) (fail_cond : uact)
+                       (rir' : rule_information_raw) (nid' : nat)
+                       (vvs0 : list (string * uact)),
+                  wf_uact_known_vars (map fst env) u ->
+                  get_rule_information_aux u env vvs0 guard rir nid =
+                    (v, env', vvs, fail_cond, rir', nid') ->
+                  Forall2 (fun x y : string * string => fst x = fst y) env env') args
+      )
+      names0 vvs0 fail0 rir nid l0 env' l u r n guard,
+      gria_list' guard get_rule_information_aux args env vvs0 rir nid names0 fail0 =
+        (l0, env', l, u, r, n) ->
+      Forall2 (fun x y => fst x = fst y) env env' /\ List.length l0 = List.length names0 + List.length args.
+  Proof.
+    induction args; simpl; intros; eauto.
+    - inv H. split. apply same_env_refl. lia.
+    - repeat destr_in H. subst. inv IH. inv F.
+      eapply H2 in Heqp; eauto. clear H2.
+      eapply IHargs in H; eauto.
+      destruct H.
+      split.
+      eapply same_env_trans; eauto. congruence.
+      simpl in H0. lia.
+      erewrite <- same_env_same_fst; eauto.
+  Qed.
+
+  Lemma map_fst_combine:
+    forall {A B: Type} (l1: list A) (l2: list B),
+      List.length l1 = List.length l2 ->
+      map fst (combine l1 l2) = l1.
+  Proof.
+    induction l1; simpl; intros; eauto. destr. simpl in *; lia. simpl in *.
+    f_equal. eauto.
+  Qed.
+
+  Lemma fst_split_map:
+    forall {A B: Type} (l: list (A*B)),
+      fst (split l) = map fst l.
+  Proof.
+    induction l; simpl; intros; eauto. repeat destr. subst. simpl. f_equal.
+    simpl in IHl. auto.
+  Qed.
+  
+  Lemma get_rule_information_aux_same_vm:
+    forall (ua: uact)
+           (env: list (string * string)) (guard: uact)
+           (rir: rule_information_raw) (nid: nat)
+           v env' vvs fail_cond rir' nid' vvs0
+           (WUKV: wf_uact_known_vars (map fst env) ua)
+           (GRIA: get_rule_information_aux ua env vvs0 guard rir nid = (v, env', vvs, fail_cond, rir', nid'))
+    ,
+      Forall2 (fun x y => fst x = fst y) env env'.
+  Proof.
+    assert (forall e : list (string*string), Forall2 (fun x y => fst x = fst y) e e).
+    {
+      induction e; simpl; intros; eauto.
+    }
+    Opaque skipn.
+    intros ua; pattern ua; eapply daction_ind'; simpl; intros; eauto.
+    all: try now (repeat destr_in GRIA; inv GRIA; inv WUKV; eauto).
+    - repeat destr_in GRIA; inv GRIA; inv WUKV; eauto.
+      apply H0 in Heqp; auto.
+      eapply same_env_set_in; eauto.
+    - repeat destr_in GRIA; inv GRIA; inv WUKV; eauto.
+      apply H0 in Heqp; auto.
+      apply H1 in Heqp4; auto.
+      eapply same_env_trans; eauto. congruence.
+      erewrite <- same_env_same_fst; eauto.
+    - repeat destr_in GRIA. inv GRIA.
+      apply H0 in Heqp; auto.
+      apply H1 in Heqp4; auto.
+      inv Heqp4. eauto.
+      inv WUKV. simpl; auto.
+      inv WUKV. auto.
+    - do 17 destr_in GRIA. inv GRIA; inv WUKV; eauto.
+      apply H0 in Heqp; auto.
+      apply H1 in Heqp4; auto.
+      apply H2 in Heqp9; auto.
+      eapply same_env_trans; eauto. congruence.
+      eapply merge_vms_preserve_same_env in Heqp14.
+      eapply same_env_trans. congruence. apply Heqp4. auto.
+      eapply same_env_trans. congruence. apply same_env_sym. eauto. auto.
+      erewrite <- same_env_same_fst; eauto.
+      erewrite <- same_env_same_fst; eauto.
+    - repeat destr_in GRIA. inv GRIA. inv WUKV.
+      apply H0 in Heqp; auto.
+      apply H1 in Heqp4; auto.
+      eapply same_env_trans; eauto. congruence.
+      erewrite <- same_env_same_fst; eauto.
+    - repeat destr_in GRIA. inv GRIA. inv WUKV.
+      eapply gria_list_same_env in Heqp; eauto.
+      destruct Heqp; eauto.
+  Qed.
+
+  Lemma in_list_assoc_set_inv:
+    forall {K V: Type} {eq_dec: EqDec K} (l: list (K * V)) k' v' k v,
+      In (k', v') (list_assoc_set l k v) ->
+      (k, v) = (k', v') \/ In (k', v') l.
+  Proof.
+    induction l; simpl; intros; eauto.
+    repeat destr_in H; simpl in *; subst.
+    destruct H; auto.
+    destruct H; auto. apply IHl in H. destruct H; auto.
+  Qed.
+
+  Definition valid_name name nid :=
+    exists n, name = generate_binding_name n /\ n < nid.
+  Definition vvs_range (vvs: list (string * uact)) (nid: nat) :=
+    forall x y,
+      In (x,y) vvs -> valid_name x nid.
+
+  Lemma string_append_inj:
+    forall (s1 s2 s3: string),
+      String.append s1 s2 = String.append s1 s3 -> s2 = s3.
+  Proof.
+    induction s1; simpl; intros; eauto. inv H. eauto.
+  Qed.
+  Lemma generate_binding_name_inj:
+    forall n1 n2,
+      generate_binding_name n1 = generate_binding_name n2 -> n1 = n2.
+  Proof.
+    unfold generate_binding_name.
+
+    intros.
+    apply string_append_inj in H.
+    apply (f_equal NilEmpty.uint_of_string) in H.
+    rewrite ! NilEmpty.usu in H.
+    inv H.
+  Admitted.
+
+  Lemma list_assoc_set_not_before:
+    forall {K V: Type} {eqdec: EqDec K} (l: list (K * V)) k v k' v' ,
+      ~ In k (map fst l) ->
+      In (k', v') (list_assoc_set l k v) <-> In (k', v') l \/ (k, v) = (k', v').
+  Proof.
+    induction l; simpl; intros; eauto. tauto.
+    repeat destr; simpl in *; subst.
+    contradict H. auto.
+    rewrite IHl. tauto. tauto.
+  Qed.
+
+  Lemma vvs_range_in_fst:
+    forall vvs n,
+    vvs_range vvs n ->
+    forall k,
+      In (generate_binding_name k) (map fst vvs) ->
+      k < n.
+  Proof.
+    unfold vvs_range. intros.
+    rewrite in_map_iff in H0. destruct H0 as (x & EQ & IN).
+    destruct x. simpl in *. subst.
+    apply H in IN.
+    destruct IN as (n0 & EQ & LT).
+    apply generate_binding_name_inj in EQ. subst. auto.
+  Qed.
+
+  Lemma vvs_range_list_assoc_set:
+    forall vvs n name v,
+      vvs_range vvs n ->
+      valid_name name n ->
+      vvs_range (list_assoc_set vvs name v) n.
+  Proof.
+    unfold vvs_range; simpl; intros.
+    apply in_list_assoc_set_inv in H1; destruct H1. inv H1. auto. eauto.
+  Qed.
+
+  Lemma valid_name_incr:
+    forall name n1 n2 (INCR: n1 <= n2),
+      valid_name name n1 -> valid_name name n2.
+  Proof.
+    unfold valid_name. intros name n1 n2 INCR (n & EQ & LT).
+    eexists; split; eauto. lia.
+  Qed.
+
+  Lemma vvs_range_incr:
+    forall vvs n1 n2 (INCR: n1 <= n2),
+      vvs_range vvs n1 -> vvs_range vvs n2.
+  Proof.
+    unfold vvs_range; simpl; intros; eauto using valid_name_incr.
+  Qed.
+  Ltac trim H :=
+    match type of H with
+    | ?a -> ?b =>
+      let x := fresh "H" in
+      assert(x: a);[|specialize(H x); clear x]
+    end.
+
+  Lemma in_map_list_assoc_set_inv:
+    forall {K V: Type} {eqdec: EqDec K} (l : list (K * V)) (k : K)
+           (v : V) k' ,
+      In k' (map fst (list_assoc_set l k v)) ->
+      k = k' \/ In k' (map fst l).
+  Proof.
+    induction l; simpl; intros; eauto. repeat destr_in H. subst. simpl. auto.
+    simpl in *. destruct H; auto. apply IHl in H. tauto.
+  Qed.
+
+
+  Definition var_lt (v1 v2: string) :=
+    exists n1 n2,
+      v1 = generate_binding_name n1
+      /\ v2 = generate_binding_name n2
+      /\ n1 < n2.
+
+  Lemma var_lt_gen_r:
+    forall s n n' ,
+      n <= n' ->
+      var_lt s (generate_binding_name n) ->
+      var_lt s (generate_binding_name n').
+  Proof.
+    unfold var_lt; simpl; intros. destruct H0 as (n1 & n2 & EQ & EQ2 & LT). subst.
+    apply generate_binding_name_inj in EQ2.
+    do 2 eexists; repeat split; eauto. lia.
+  Qed.
+
+  Lemma merge_banches_grows:
+    forall vm_tb vm_fb vvs nid cond_name vm' vvs' nid'
+           (MB: merge_branches' vm_tb vm_fb vvs nid cond_name = (vm', vvs', nid'))
+           (ENVVVS1: forall x y, In (x,y) vm_tb -> In y (map fst vvs))
+           (ENVVVS2: forall x y, In (x,y) vm_fb -> In y (map fst vvs))
+           (RNGVVS: vvs_range vvs nid)
+           (VVSVALID: forall (v : string) (a : uact),
+               In (v, a) vvs -> forall v' : string, var_in_uact a v' -> var_lt v' v
+           )
+           (VALIDCOND: valid_name cond_name nid)
+    ,
+      (forall x y, In (x,y) vvs -> In (x,y) vvs') /\
+        vvs_range vvs' nid' /\
+        (forall x y, In (x,y) vm' -> In y (map fst vvs')) /\ nid <= nid' /\
+        (forall (v : string) (a : uact),
+            In (v, a) vvs' -> forall v' : string, var_in_uact a v' -> var_lt v' v).
+  Proof.
+    induction vm_tb; simpl; intros; eauto.
+    - inv MB. split; auto.
+    - repeat destr_in MB; inv MB. auto.
+      + edestruct IHvm_tb as (VVSGROWS3 & VVSRANGE3 & ENVVVS3 & NIDGROWS3 & VVSVALID3). eauto.
+        intros; eapply ENVVVS1; eauto.
+        intros; eapply ENVVVS2; simpl; eauto. auto. auto. auto.
+        repeat split; auto.
+        simpl; intros. destruct H; eauto. inv H.
+        specialize (ENVVVS2 _ _ (or_introl eq_refl)). apply in_map_iff in ENVVVS2.
+        destruct ENVVVS2 as ((s3&aa)&EQ&IN). simpl in *; subst.
+        apply VVSGROWS3 in IN.
+        apply (in_map fst) in IN. simpl in IN.
+        apply eqb_eq in Heqb. subst; auto.
+      + edestruct IHvm_tb as (VVSGROWS3 & VVSRANGE3 & ENVVVS3 & NIDGROWS3 & VVSVALID3). eauto.
+        intros; eapply ENVVVS1; eauto.
+        intros; eapply ENVVVS2; simpl; eauto. auto. auto. auto.
+        repeat split; auto.
+        * simpl; intros. rewrite in_app_iff. eauto.
+        * red. intros x y. rewrite in_app_iff.  intros [A|A].
+          eapply VVSRANGE3 in A. eapply valid_name_incr. 2: eauto. lia.
+          simpl in A. destruct A as [A|[]]. inv A. red; eexists; split; eauto.
+        * simpl. intros x y [A|A].
+          inv A. rewrite map_app.  apply in_or_app. right. simpl.  auto.
+          rewrite map_app.  apply in_or_app. left. eauto.
+        * intros.
+          rewrite in_app_iff in H. destruct H; eauto.
+          simpl in H. destruct H as [H|[]]. inv H.
+          inv H0. inv H4.
+          destruct VALIDCOND as (condno & EQ & LT). subst.
+          do 2 eexists; repeat split; eauto. lia.
+          inv H4; eauto.
+          specialize (ENVVVS2 _ _ (or_introl eq_refl)). apply in_map_iff in ENVVVS2.
+          destruct ENVVVS2 as ((ss&a) & EQ & IN). simpl in *. subst.
+          apply RNGVVS in IN.
+          destruct IN as (condno & EQ & LT). subst.
+          do 2 eexists; repeat split; eauto. lia.
+          inv H4; eauto.
+          specialize (ENVVVS1 _ _ (or_introl eq_refl)). apply in_map_iff in ENVVVS1.
+          destruct ENVVVS1 as ((ss&a) & EQ & IN). simpl in *. subst.
+          apply RNGVVS in IN.
+          destruct IN as (condno & EQ & LT). subst.
+          do 2 eexists; repeat split; eauto. lia.
+  Qed.
+
+  Definition valid_vars_uact v n :=
+    forall var, var_in_uact v var -> var_lt var (generate_binding_name n).
+  Lemma valid_vars_merge_failures:
+    forall u u0 n,
+      valid_vars_uact u n ->
+      valid_vars_uact u0 n ->
+      valid_vars_uact (merge_failures u u0) n.
+  Proof.
+    red; intros. inv H1; eauto.
+  Qed.
+
+  Lemma valid_vars_and:
+    forall u u0 n,
+      valid_vars_uact u n ->
+      valid_vars_uact u0 n ->
+      valid_vars_uact (uand u u0) n.
+  Proof.
+    red; intros. inv H1; eauto.
+  Qed.
+
+  Lemma valid_vars_not:
+    forall u n,
+      valid_vars_uact u n ->
+      valid_vars_uact (unot u) n.
+  Proof.
+    red; intros. inv H0; eauto.
+  Qed.
+
+  Lemma valid_vars_fold_uor:
+    forall conds n,
+      Forall (fun a => valid_vars_uact a n) conds ->
+      forall ci,
+        valid_vars_uact ci n ->
+        valid_vars_uact (fold_left uor conds ci) n.
+  Proof.
+    induction 1; simpl; intros; eauto.
+    apply IHForall. apply valid_vars_merge_failures; auto.
+  Qed.
+
+  Lemma valid_vars_or_conds:
+    forall conds n,
+      Forall (fun a => valid_vars_uact a n) conds ->
+      valid_vars_uact (or_conds conds) n.
+  Proof.
+    intros; eapply valid_vars_fold_uor; eauto.
+    red; intros. inv H0.
+  Qed.
+
+  Lemma valid_var_uact_incr:
+    forall v n1 n2,
+      valid_vars_uact v n1 ->
+      n1 <= n2 ->
+      valid_vars_uact v n2.
+  Proof.
+    red; intros.
+    eapply H in H1. eapply var_lt_gen_r; eauto.
+  Qed.
+
+  Lemma gria_list_grows:
+    forall
+      (I: list (string*string) -> list (string * uact) -> nat -> rule_information_raw -> uact -> Prop)
+      (P: list (string*string) -> list (string * uact) -> nat -> rule_information_raw ->
+          list (string*string) -> list (string * uact) -> nat -> rule_information_raw -> Prop)
+      (Prefl: forall env vvs nid rir, P env vvs nid rir env vvs nid rir)
+      (Ptrans: forall env1 vvs1 nid1 rir1 env2 vvs2 nid2 rir2 env3 vvs3 nid3 rir3 grd1 grd2,
+          I env1 vvs1 nid1 rir1 grd1 ->
+          P env1 vvs1 nid1 rir1 env2 vvs2 nid2 rir2 ->
+          I env2 vvs2 nid2 rir2 grd2 ->
+          P env2 vvs2 nid2 rir2 env3 vvs3 nid3 rir3 ->
+          P env1 vvs1 nid1 rir1 env3 vvs3 nid3 rir3
+      )
+      (Pwukv:
+        forall env1 vvs1 nid1 rir1 env2 vvs2 nid2 rir2,
+          P env1 vvs1 nid1 rir1 env2 vvs2 nid2 rir2 ->
+          forall u,
+            wf_uact_known_vars (map fst env1) u ->
+            wf_uact_known_vars (map fst env2) u
+      )
+      (Psetvvs:
+        forall env vvs n rir grd v,
+          I env vvs n rir grd ->
+          valid_vars_uact v n ->
+          P env vvs n rir env (list_assoc_set vvs (generate_binding_name n) v) (S n) rir /\
+            I env (list_assoc_set vvs (generate_binding_name n) v) (S n) rir grd
+      )
+      (Pvvsgrows:
+        forall env1 vvs1 nid1 rir1 grd1 env2 vvs2 nid2 rir2,
+          P env1 vvs1 nid1 rir1 env2 vvs2 nid2 rir2 ->
+          I env1 vvs1 nid1 rir1 grd1 ->
+          forall x,
+            In x (map fst vvs1) -> In x (map fst vvs2)
+      )
+      rec args
+      (F: Forall (fun u =>
+                    forall env guard rir nid v env' vvs fail_cond rir' nid' vvs0,
+                      rec u env vvs0 guard rir nid = (v, env', vvs, fail_cond, rir', nid') ->
+                      wf_uact_known_vars (map fst env) u ->
+                      valid_vars_uact guard nid ->
+                      I env vvs0 nid rir guard ->
+                      P env vvs0 nid rir env' vvs nid' rir' /\ I env' vvs nid' rir' guard
+                      /\ (forall ov, v = Some ov -> valid_vars_uact ov nid')
+                      /\ valid_vars_uact guard nid'
+                      /\ valid_vars_uact fail_cond nid'
+                      /\ nid <= nid'
+                 ) args)
+      guard env vvs0 rir nid names0 fail0 names env' vvs fail1 rir' nid'
+      (WUKV: Forall (wf_uact_known_vars (map fst env)) args)
+      (VG: valid_vars_uact guard nid)
+      (VF: valid_vars_uact fail0 nid)
+      (INV: I env vvs0 nid rir guard)
+      (GRIA: gria_list' guard rec args env vvs0 rir nid names0 fail0 = (names, env', vvs, fail1, rir', nid'))
+      (NAMES: Forall (fun name => In name (map fst vvs0)) names0)
+    ,
+      P env vvs0 nid rir env' vvs nid' rir'
+      /\ I env' vvs nid' rir' guard
+      /\ Forall (fun name => In name (map fst vvs)) names
+      /\ List.length names = List.length names0 + List.length args
+      /\ valid_vars_uact fail1 nid'
+      /\ nid <= nid'.
+  Proof.
+    induction 6; simpl; intros; eauto.
+    - inv GRIA. repeat split; eauto.
+    - inv WUKV.
+      repeat destr_in GRIA. subst.
+      apply H in Heqp; auto. destruct Heqp as (P2 & I2 & RV2 & VG2 & VF2 & NIDGROWS2). clear H.
+      eapply Forall_impl in H3.
+      2: intros a WUKV; eapply Pwukv in WUKV. 3: exact P2. 2: apply WUKV.
+      eapply IHF in GRIA;  eauto.
+      destruct GRIA as (Pgria & Igria & NAMES1 & LENNAMES & VF3 & NIDGROWS).
+
+      repeat split; eauto.
+      + eapply Ptrans; eauto.
+        eapply Ptrans. eauto. 3: eauto.
+        all: eapply Psetvvs; eauto.
+        intros. destruct o. simpl. eauto. red; simpl; intros. inv H.
+        intros. destruct o. simpl. eauto. red; simpl; intros. inv H.
+      + simpl in LENNAMES; lia.
+      + lia.
+      + red; intros. eapply var_lt_gen_r. 2: eauto. lia.
+      + eapply valid_vars_merge_failures; eauto using valid_var_uact_incr.
+      + eapply Psetvvs; eauto.
+        intros. destruct o. simpl. eauto. red; simpl; intros. inv H.
+      + constructor.
+        apply list_assoc_set_key_in.
+        eapply Forall_impl. 2: apply NAMES. simpl.
+        intros a IN.
+        eapply Pvvsgrows in IN. 2: eauto.
+        eapply list_assoc_set_key_stays_in; eauto. eauto.
+  Qed.
+
+  Lemma list_assoc_in:
+    forall {K V: Type} {eq_dec_k: EqDec K} (l: list (K*V)) k v,
+      list_assoc l k = Some v -> In (k,v) l.
+  Proof.
+    induction l; simpl; intros; eauto. easy. repeat destr_in H. inv H. auto. eauto.
+  Qed.
+
+  Lemma incl_incl_map:
+    forall {A B: Type} (l1 l2: list (A * B))
+           (P: forall x y, In (x, y) l1 -> In (x, y) l2),
+    forall x, In x (map fst l1) -> In x (map fst l2).
+  Proof.
+    intros.
+    rewrite in_map_iff in H.
+    destruct H as ((a,b) & EQ & IN). subst.
+    apply in_map; auto.
+  Qed.
+
+
+  Record wf_write_log_raw (wl: write_log_raw) (n: nat) :=
+    {
+      wf_wlr_glob_cond: forall i a, In (i, a) wl -> valid_vars_uact (fst a) n ;
+      wf_wlr_each_cond: forall i a, In (i, a) wl ->
+                                    Forall (fun wi => valid_vars_uact (wcond wi) n) (snd a);
+      wf_wlr_each_act: forall i a, In (i, a) wl ->
+                                   Forall (fun wi => valid_vars_uact (wval wi) n) (snd a);
+    }.
+
+  Record wf_extcall_info (ext: extcall_info) (n: nat) :=
+    {
+      wf_ei_cond: valid_vars_uact (econd ext) n;
+      wf_ei_arg: valid_vars_uact (earg ext) n;
+      wf_ei_bind: var_lt (ebind ext) (generate_binding_name n);
+    }.
+
+  Record wf_rir (r: rule_information_raw) (n: nat) :=
+    {
+      wf_rir_read0s: forall i a, In (i, a) (rir_read0s r) -> valid_vars_uact a n;
+      wf_rir_read1s: forall i a, In (i, a) (rir_read1s r) -> valid_vars_uact a n;
+      wf_rir_write0s: wf_write_log_raw (rir_write0s r) n;
+      wf_rir_write1s: wf_write_log_raw (rir_write1s r) n;
+      wf_rir_extcalls: forall i ext, In (i, ext) (rir_extcalls r) -> wf_extcall_info ext n
+    }.
+
+
+  Lemma wf_extcall_info_incr:
+    forall r n1 n2,
+      wf_extcall_info r n1 ->
+      n1 <= n2 ->
+      wf_extcall_info r n2.
+  Proof.
+    intros. inv H. split; eauto using valid_var_uact_incr.
+    eauto using var_lt_gen_r.
+  Qed.
+
+  Lemma wf_write_log_raw_incr:
+    forall r n1 n2,
+      wf_write_log_raw r n1 ->
+      n1 <= n2 ->
+      wf_write_log_raw r n2.
+  Proof.
+    intros. inv H. split; eauto using valid_var_uact_incr.
+    intros. apply wf_wlr_each_cond0 in H. eapply Forall_impl; eauto. simpl; eauto using valid_var_uact_incr.
+    intros. apply wf_wlr_each_act0 in H. eapply Forall_impl; eauto. simpl; eauto using valid_var_uact_incr.
+  Qed.
+
+  Lemma wf_rir_incr:
+    forall r n1 n2,
+      wf_rir r n1 ->
+      n1 <= n2 ->
+      wf_rir r n2.
+  Proof.
+    intros. inv H. split; eauto using valid_var_uact_incr, wf_extcall_info_incr, wf_write_log_raw_incr.
+  Qed.
+
+  Lemma vss_or_extcall_var_lt:
+    forall l n rir
+           (VVSRANGE : vvs_range l n)
+           (RIRRNG : wf_rir rir n)
+           v'
+           (H0 : In v' (map fst l) \/
+                   (exists ext : ext_fn_t * extcall_info,
+                       In ext (rir_extcalls rir) /\ ebind (snd ext) = v')),
+      var_lt v' (generate_binding_name n).
+  Proof.
+    intros.
+    destruct H0.
+    rewrite in_map_iff in H. destruct H as ((s&a) & EQ & IN). apply VVSRANGE in IN.
+    red in IN. destruct IN as (n0 & EQ2 & LT). do 2 eexists; repeat split; eauto. subst.  reflexivity.
+    destruct H as (ext & IN & EQ).
+    subst. inv RIRRNG. destruct ext. apply wf_rir_extcalls0 in IN.
+    destruct IN. eauto.
+  Qed.
+
+
+  Lemma filter_map_In:
+    forall {A B: Type} (f: A -> option B) l x,
+      In x (filter_map f l) <-> (exists y, Some x = f y /\ In y l).
+  Proof.
+    induction l; simpl; intros; eauto. split. tauto. intros (y & _ & []).
+    destr; simpl; rewrite IHl.
+    - split. intros [C | (y & EQ & IN)]. subst. eexists; split; eauto.
+      eexists; split; eauto.
+      intros (y & EQ & [IN|IN]); subst. left; congruence. right; eexists; split; eauto.
+    - split; intros (y & EQ & IN); eauto.
+      destruct IN as [IN|IN]; eauto. congruence.
+  Qed.
+
+  Lemma Forall_list_options:
+    forall {A:Type} (P: A -> Prop) l,
+      (forall x y,
+          In x l ->
+          x = Some y ->
+          P y
+      ) ->
+      Forall P (filter_map id l).
+  Proof.
+    intros.
+    rewrite Forall_forall. intros.
+    rewrite filter_map_In in H0. destruct H0 as (y & EQ & IN). unfold id in EQ. subst.
+    eauto.
+  Qed.
+
+  Lemma wf_rir_add_write0:
+    forall rir n guard v idx rir' fail,
+      wf_rir rir n ->
+      valid_vars_uact guard n ->
+      valid_vars_uact v n ->
+      add_write0 rir guard idx v = (rir', fail) ->
+      wf_rir rir' n /\ valid_vars_uact fail n.
+  Proof.
+    intros. inv H. unfold add_write0 in H2.
+    repeat destr_in H2. inv H2.
+    split. repeat (split; simpl; eauto).
+    - intros i a IN.
+      apply in_list_assoc_set_inv in IN. destruct IN; eauto.
+      inv H. simpl. destr_in Heqp; inv Heqp; eauto.
+      apply list_assoc_in in Heqo.
+      destruct p; simpl in *. apply valid_vars_merge_failures; eauto.
+      inv wf_rir_write0s0. eapply wf_wlr_glob_cond0 in Heqo; eauto.
+      eapply wf_wlr_glob_cond in H; eauto.
+    - intros i a IN.
+      apply in_list_assoc_set_inv in IN. destruct IN; eauto.
+      inv H. simpl. destr_in Heqp; inv Heqp; eauto.
+      apply Forall_app; split; eauto.
+      apply list_assoc_in in Heqo.
+      destruct p; simpl in *. eapply wf_wlr_each_cond in Heqo; eauto.
+      eapply wf_wlr_each_cond in H; eauto.
+    - intros i a IN.
+      apply in_list_assoc_set_inv in IN. destruct IN; eauto.
+      inv H. simpl. destr_in Heqp; inv Heqp; eauto.
+      apply Forall_app; split; eauto.
+      apply list_assoc_in in Heqo.
+      destruct p; simpl in *. eapply wf_wlr_each_act in Heqo; eauto.
+      eapply wf_wlr_each_act in H; eauto.
+    - apply valid_vars_and. auto.
+      apply valid_vars_or_conds.
+      apply Forall_list_options. simpl. intros. subst. unfold option_map in H.
+      destruct H as [H|[H|[H|[]]]]; repeat destr_in H; inv H.
+      + destruct p. apply list_assoc_in in Heqo.
+        eapply wf_wlr_glob_cond in Heqo; eauto.
+      + apply list_assoc_in in H3.
+        eapply wf_rir_read1s0 in H3. auto.
+      + destruct p. apply list_assoc_in in Heqo.
+        eapply wf_wlr_glob_cond in Heqo; eauto.
+  Qed.
+
+  Lemma wf_rir_add_write1:
+    forall rir n guard v idx rir' fail,
+      wf_rir rir n ->
+      valid_vars_uact guard n ->
+      valid_vars_uact v n ->
+      add_write1 rir guard idx v = (rir', fail) ->
+      wf_rir rir' n /\ valid_vars_uact fail n.
+  Proof.
+    intros. inv H. unfold add_write1 in H2.
+    repeat destr_in H2. inv H2.
+    split. repeat (split; simpl; eauto).
+    - intros i a IN.
+      apply in_list_assoc_set_inv in IN. destruct IN; eauto.
+      inv H. simpl. destr_in Heqp; inv Heqp; eauto.
+      apply list_assoc_in in Heqo.
+      destruct p; simpl in *. apply valid_vars_merge_failures; eauto.
+      inv wf_rir_write1s0. eapply wf_wlr_glob_cond0 in Heqo; eauto.
+      eapply wf_wlr_glob_cond in H; eauto.
+    - intros i a IN.
+      apply in_list_assoc_set_inv in IN. destruct IN; eauto.
+      inv H. simpl. destr_in Heqp; inv Heqp; eauto.
+      apply Forall_app; split; eauto.
+      apply list_assoc_in in Heqo.
+      destruct p; simpl in *. eapply wf_wlr_each_cond in Heqo; eauto.
+      eapply wf_wlr_each_cond in H; eauto.
+    - intros i a IN.
+      apply in_list_assoc_set_inv in IN. destruct IN; eauto.
+      inv H. simpl. destr_in Heqp; inv Heqp; eauto.
+      apply Forall_app; split; eauto.
+      apply list_assoc_in in Heqo.
+      destruct p; simpl in *. eapply wf_wlr_each_act in Heqo; eauto.
+      eapply wf_wlr_each_act in H; eauto.
+    - apply valid_vars_and. auto.
+      apply valid_vars_or_conds.
+      apply Forall_list_options. simpl. intros. subst. unfold option_map in H.
+      destruct H as [H|[]]; repeat destr_in H; inv H.
+      destruct p. apply list_assoc_in in Heqo.
+      eapply wf_wlr_glob_cond in Heqo; eauto.
+  Qed.
+
+  Lemma wf_rir_add_read0:
+    forall rir n guard idx,
+      wf_rir rir n ->
+      valid_vars_uact guard n ->
+      wf_rir (add_read0 rir guard idx) n.
+  Proof.
+    intros. inv H. unfold add_read0. split; simpl; eauto.
+    intros.
+    apply in_list_assoc_set_inv in H. destruct H.
+    - inv H. destr; eauto.
+      apply valid_vars_merge_failures; auto.
+      apply list_assoc_in in Heqo. eauto.
+    - eauto.
+  Qed.
+  Lemma wf_rir_add_read1:
+    forall rir n guard idx,
+      wf_rir rir n ->
+      valid_vars_uact guard n ->
+      wf_rir (add_read1 rir guard idx) n.
+  Proof.
+    intros. inv H. unfold add_read1. split; simpl; eauto.
+    intros.
+    apply in_list_assoc_set_inv in H. destruct H.
+    - inv H. destr; eauto.
+      apply valid_vars_merge_failures; auto.
+      apply list_assoc_in in Heqo. eauto.
+    - eauto.
+  Qed.
+
+  Lemma get_rule_information_aux_env_grows:
+    forall (ua: uact)
+           (env: list (string * string)) (guard: uact)
+           (rir: rule_information_raw) (nid: nat)
+           v env' vvs fail_cond rir' nid' vvs0
+           (GRIA: get_rule_information_aux ua env vvs0 guard rir nid = (v, env', vvs, fail_cond, rir', nid'))
+           (WUKV: wf_uact_known_vars (map fst env) ua)
+           (ENVVVS: forall x y, In (x,y) env -> In y (map fst vvs0))
+           (RNGVVS: vvs_range vvs0 nid)
+           (VVSVALID: forall v a, In (v, a) vvs0 -> forall v' , var_in_uact a v' -> var_lt v' v)
+           (RIRRNG: wf_rir rir nid)
+           (GUARDVALID: valid_vars_uact guard nid),
+      (forall x y, In (x,y) vvs0 -> In (x,y) vvs)
+      /\ vvs_range vvs nid'
+      /\ (forall x y, In (x,y) env' -> In y (map fst vvs))
+      /\ (forall ext, In ext (rir_extcalls rir) -> In ext (rir_extcalls rir'))
+      /\ (forall ov x, v = Some ov -> var_in_uact ov x ->
+                       In x (map fst vvs) \/
+                         exists ext, In ext (rir_extcalls rir') /\ ebind (snd ext) = x)
+      /\ wf_rir rir' nid'
+      /\ (forall v a, In (v, a) vvs -> forall v' , var_in_uact a v' -> var_lt v' v)
+      /\ valid_vars_uact fail_cond nid'
+      /\ nid <= nid'
+  .
+  Proof.
+    intros ua; pattern ua; eapply daction_ind'; simpl; intros; eauto.
+    all: repeat destr_in GRIA; inv GRIA; inv WUKV; eauto; try now (intuition congruence).
+    - intuition try congruence. red; intros. inv H. lia.
+    - intuition try congruence. red; intros. inv H. lia.
+    - intuition try congruence.
+      inv H. inv H0. apply list_assoc_in in Heqo. eauto.
+      red; intros. inv H.
+      lia.
+    - intuition try congruence. red; intros. inv H. lia.
+    - intuition try congruence. inv H. inv H0. red; intros. inv H. lia.
+    - specialize (H _ _ _ _ _ _ _ _ _ _ _ Heqp H3 ENVVVS RNGVVS VVSVALID RIRRNG GUARDVALID).
+      destruct H as (VVSGROWS & VVSRANGE & ENVVVS2 & EXTCALL2 & VAR2 & RIRLT2 & LT2 & VF2 & GUARDVALID2).
+      repeat (refine (conj _ _)); eauto.
+      + intros.
+        rewrite list_assoc_set_not_before. eauto. intro IN.
+        eapply vvs_range_in_fst in IN. 2: eauto. lia.
+      + eapply vvs_range_list_assoc_set. eapply vvs_range_incr. 2: eauto. lia.
+        red. eexists; split; eauto.
+      + intros.
+        apply in_list_assoc_set_inv in H.
+        destruct H. inv H.
+        eapply list_assoc_set_key_in; eauto.
+        apply ENVVVS2 in H.
+        eapply list_assoc_set_key_stays_in; eauto.
+      + easy.
+      + eapply wf_rir_incr; eauto.
+      + intros.
+        apply in_list_assoc_set_inv in H. destruct H; eauto.
+        inv H.
+        destruct o; simpl in H0; [| inv H0].
+        eapply VAR2 in H0; eauto.
+        eapply vss_or_extcall_var_lt in H0. eauto. auto. eauto.
+      + eapply valid_var_uact_incr; eauto.
+    - specialize (H0 _ _ _ _ _ _ _ _ _ _ _ Heqp4).
+      specialize (H _ _ _ _ _ _ _ _ _ _ _ Heqp H4).
+      generalize (get_rule_information_aux_same_vm _ _ _ _ _ _ _ _ _ _ _ _ H4 Heqp).
+      generalize (fun wukv => get_rule_information_aux_same_vm _ _ _ _ _ _ _ _ _ _ _ _ wukv Heqp4).
+      intros SVM2 SVM1.
+      erewrite same_env_same_fst in H5. 2: eauto.
+      specialize (SVM2 H5).
+      specialize (H0 H5).
+      specialize (H ENVVVS RNGVVS VVSVALID RIRRNG GUARDVALID).
+      destruct H as (VVSGROWS1 & VVSRANGE1 & ENVVVS1 & EXTCALL1 & VAR1 & RIRRNG1 & VVSVALID1 & VF1 & GV1).
+      specialize (H0 ENVVVS1 VVSRANGE1).
+      destruct H0 as (VVSGROWS2 & VVSRANGE2 & ENVVVS2 & EXTCALL2 &  VAR2 & RIRRNG2 & VVSVALID2 & VF2 & GV2); eauto.
+      2: repeat refine (conj _ _); eauto.
+      eapply valid_var_uact_incr; eauto.
+
+      red; intros. inv H. eapply VF1 in H6. eapply var_lt_gen_r; eauto.
+      eauto.
+      lia.
+
+    - specialize (H0 _ _ _ _ _ _ _ _ _ _ _ Heqp4).
+      specialize (H _ _ _ _ _ _ _ _ _ _ _ Heqp).
+      generalize (get_rule_information_aux_same_vm _ _ _ _ _ _ _ _ _ _ _ _ H4 Heqp).
+      generalize (fun wukv => get_rule_information_aux_same_vm _ _ _ _ _ _ _ _ _ _ _ _ wukv Heqp4). simpl.
+      intros SVM2 SVM1.
+      specialize (SVM2 H6). inv SVM2. simpl in H3. subst.
+      simpl in *.
+      change (skipn 1 (y::l')) with l'.
+      specialize (H H4 ENVVVS RNGVVS VVSVALID RIRRNG).
+      destruct H as (VVSGROWS1 & VVSRANGE1 & ENVVVS1 & EXTCALL1 & VAR1 & RIRRNG1 & VVSVALID1 & VF1 & GV1); eauto.
+      specialize (H0 H6). destruct y; simpl in *.
+      trim H0.
+      {
+        intros x y [A|A].
+        - inv A.
+          apply list_assoc_set_key_in.
+        - eapply list_assoc_set_key_stays_in.
+          apply ENVVVS in A. rewrite in_map_iff in A. destruct A as ((x0&x1) & EQ & A). simpl in EQ; subst.
+          apply VVSGROWS1 in A.
+          apply (in_map fst) in A. simpl in A; auto.
+      }
+      trim H0.
+      apply vvs_range_list_assoc_set. eapply vvs_range_incr. 2: eauto. lia.
+      red. eauto.
+      destruct H0 as (VVSGROWS2 & VVSRANGE2 & ENVVVS2 & EXTCALL2 & VAR2 & RIRRNG2 & VVSVALID2 & VF2 & GV2).
+      {
+        intros v a IN.
+        apply in_list_assoc_set_inv in IN. destruct IN as [IN|IN]; eauto.
+        inv IN.
+        intros v' VIU.
+        destruct o; simpl in VIU; [| inv VIU].
+        eapply VAR1 in VIU; eauto.
+        eapply vss_or_extcall_var_lt in VIU. eauto. auto. eauto.
+      }
+      eapply wf_rir_incr; eauto.
+      eapply valid_var_uact_incr; eauto.
+      repeat (refine (conj _ _)); eauto.
+      intros; eapply VVSGROWS2.
+      apply VVSGROWS1 in H.
+      rewrite list_assoc_set_not_before. auto.
+      intro IN.
+      eapply vvs_range_in_fst in IN. 2: eauto. lia.
+      eapply valid_vars_merge_failures; eauto. eapply valid_var_uact_incr; eauto. lia. lia.
+    -
+      specialize (H _ _ _ _ _ _ _ _ _ _ _ Heqp H6 ENVVVS RNGVVS VVSVALID RIRRNG).
+      destruct H as (VVSGROWS1 & VVSRANGE1 & ENVVVS1 & EXTCALL1 & VAR1 & RIRRNG1 & VVSVALID1 & VF1 & NIDGROWS1). eauto.
+      generalize (get_rule_information_aux_same_vm _ _ _ _ _ _ _ _ _ _ _ _ H6 Heqp). intro SVM1.
+
+      erewrite same_env_same_fst in H7; eauto.
+      erewrite same_env_same_fst in H8; eauto.
+
+      specialize (H0 _ _ _ _ _ _ _ _ _ _ _ Heqp4).
+      destruct H0 as (VVSGROWS2 & VVSRANGE2 & ENVVVS2 & EXTCALL2 & VAR2 & RIRRNG2 & VVSVALID2 & VF2 & NIDGROWS2); eauto.
+      {
+        intros.
+        apply list_assoc_set_key_stays_in.
+        apply list_assoc_set_key_stays_in.
+        apply list_assoc_set_key_stays_in. eauto.
+      }
+      {
+        eapply vvs_range_list_assoc_set.
+        eapply vvs_range_list_assoc_set.
+        eapply vvs_range_list_assoc_set.
+        eapply vvs_range_incr. 2: eauto. lia.
+        red; eexists; split; eauto. lia.
+        red; eexists; split; eauto. lia.
+        red; eexists; split; eauto. lia.
+      }
+      {
+        intros.
+        apply in_list_assoc_set_inv in H. destruct H; eauto. inv H.
+        inv H0. eapply GUARDVALID in H5. eapply var_lt_gen_r. 2: eauto. lia.
+        inv H5. inv H3.
+        do 2 eexists; repeat split; eauto. lia.
+        apply in_list_assoc_set_inv in H. destruct H; eauto. inv H.
+        inv H0. eapply GUARDVALID in H5. eapply var_lt_gen_r. 2: eauto. lia.
+        inv H5.
+        do 2 eexists; repeat split; eauto. lia.
+        apply in_list_assoc_set_inv in H. destruct H; eauto. inv H.
+        eapply VAR1 in H0; eauto.
+        eapply vss_or_extcall_var_lt in H0. eauto. auto. eauto.
+      }
+      eapply wf_rir_incr; eauto. lia.
+      {
+        red; intros. inv H.
+        do 2 eexists; repeat split; eauto. lia.
+      }
+      specialize (H1 _ _ _ _ _ _ _ _ _ _ _ Heqp9).
+      destruct H1 as (VVSGROWS3 & VVSRANGE3 & ENVVVS3 & EXTCALL3 & VAR3 & RIRRNG3 & VVSVALID3 & VF3 & NIDGROWS3). auto.
+      {
+        intros.
+        apply ENVVVS1 in H.
+        rewrite in_map_iff in H. destruct H as ((s&a)&EQ & IN). simpl in EQ. subst.
+        replace y with (fst (y, a)). eapply in_map. apply VVSGROWS2.
+        rewrite list_assoc_set_not_before.
+        rewrite list_assoc_set_not_before.
+        rewrite list_assoc_set_not_before. auto.
+        intro IN2; eapply vvs_range_in_fst in IN2; eauto. lia.
+        intro IN2. apply in_map_list_assoc_set_inv in IN2.
+        destruct IN2. apply generate_binding_name_inj in H. lia.
+        eapply vvs_range_in_fst in H; eauto. lia.
+        intro IN2. apply in_map_list_assoc_set_inv in IN2.
+        destruct IN2. apply generate_binding_name_inj in H. lia.
+        apply in_map_list_assoc_set_inv in H.
+        destruct H. apply generate_binding_name_inj in H. lia.
+        eapply vvs_range_in_fst in H; eauto. lia.
+        reflexivity.
+      }
+      auto. auto. auto.
+      {
+        red; intros. inv H.
+        do 2 eexists; repeat split; eauto. lia.
+      }
+      edestruct merge_banches_grows as (VVSGROWS4 & VVSRANGE4 & ENVVVS4 & NIDGROWS4 & VVSVALID4). eauto.
+      {
+        intros x y INl2.
+        apply ENVVVS2 in INl2.
+        rewrite in_map_iff in INl2. destruct INl2 as (xx & EQ & IN). subst. destruct xx.
+        apply VVSGROWS3 in IN. apply in_map. auto.
+      }
+      auto. auto. auto.
+      eexists; split; eauto. lia.
+      repeat (refine (conj _ _)); auto.
+      {
+        intros. eapply VVSGROWS1 in H.
+        eapply VVSGROWS4.
+        eapply VVSGROWS3.
+        eapply VVSGROWS2.
+        rewrite ! list_assoc_set_not_before. auto.
+        intro IN2; eapply vvs_range_in_fst in IN2; eauto. lia.
+        intro IN2. apply in_map_list_assoc_set_inv in IN2.
+        destruct IN2. apply generate_binding_name_inj in H0. lia.
+        eapply vvs_range_in_fst in H0; eauto. lia.
+        intro IN2. apply in_map_list_assoc_set_inv in IN2.
+        destruct IN2. apply generate_binding_name_inj in H0. lia.
+        apply in_map_list_assoc_set_inv in H0.
+        destruct H0. apply generate_binding_name_inj in H0. lia.
+        eapply vvs_range_in_fst in H0; eauto. lia.
+      }
+      {
+        intros ov x EX.
+        repeat destr_in EX; inv EX. intro VIU; inv VIU.
+        + eapply VAR1 in H3; eauto. destruct H3; eauto. left.
+          eapply incl_incl_map; eauto.
+          eapply incl_incl_map; eauto.
+          eapply incl_incl_map; eauto.
+          repeat apply list_assoc_set_key_stays_in; auto.
+          right; eauto.
+          destruct H as (ext & IN & EQ).
+          eexists; split; eauto.
+        + eapply VAR3 in H3; eauto. destruct H3; eauto. left.
+          eapply incl_incl_map; eauto.
+        + eapply VAR2 in H3; eauto. destruct H3; eauto. left.
+          eapply incl_incl_map; eauto.
+          eapply incl_incl_map; eauto.
+          destruct H as (ext & IN & EQ).
+          right; eexists; split; eauto.
+      }
+      + eapply wf_rir_incr; eauto.
+      + apply valid_vars_merge_failures.
+        eapply valid_var_uact_incr. eauto. lia.
+        apply valid_vars_merge_failures.
+        apply valid_vars_and.
+        red; intros.
+        eapply VAR1 in H. eapply vss_or_extcall_var_lt in H; eauto.
+        eapply vvs_range_incr. 2: eauto. lia.
+        eapply wf_rir_incr; eauto. lia. auto.
+        eapply valid_var_uact_incr. eauto. lia.
+        apply valid_vars_and.
+        apply valid_vars_not. 
+        red; intros.
+        eapply VAR1 in H. eapply vss_or_extcall_var_lt in H; eauto.
+        eapply vvs_range_incr. 2: eauto. lia.
+        eapply wf_rir_incr; eauto. lia. auto.
+        eapply valid_var_uact_incr. eauto. lia.
+      + lia.
+    - specialize (H _ _ _ _ _ _ _ _ _ _ _ Heqp H6 ENVVVS RNGVVS).
+      destruct H as (VVSGROWS1 & VVSRANGE1 & ENVVVS1 & EXTCALL1 & VAR1 & RIRRNG1 & VVSVALID1 & VF1 & NIDGROWS1). eauto. auto. auto.
+      generalize (get_rule_information_aux_same_vm _ _ _ _ _ _ _ _ _ _ _ _ H6 Heqp). intro SVM1.
+
+      erewrite same_env_same_fst in H7; eauto.
+      erewrite same_env_same_fst in H8; eauto.
+
+      specialize (H0 _ _ _ _ _ _ _ _ _ _ _ Heqp4).
+      destruct H0 as (VVSGROWS2 & VVSRANGE2 & ENVVVS2 & EXTCALL2 & VAR2 & RIRRNG2 & VVSVALID2 & VF2 & NIDGROWS2); auto.
+      {
+        intros.
+        apply list_assoc_set_key_stays_in.
+        apply list_assoc_set_key_stays_in.
+        apply list_assoc_set_key_stays_in. eauto.
+      }
+      {
+        eapply vvs_range_list_assoc_set.
+        eapply vvs_range_list_assoc_set.
+        eapply vvs_range_list_assoc_set.
+        eapply vvs_range_incr. 2: eauto. lia.
+        red; eexists; split; eauto. lia.
+        red; eexists; split; eauto. lia.
+        red; eexists; split; eauto. lia.
+      }
+      {
+        intros.
+        apply in_list_assoc_set_inv in H. destruct H; eauto. inv H.
+        inv H0. eapply GUARDVALID in H5. eapply var_lt_gen_r. 2: eauto. lia.
+        inv H5. inv H3.
+        do 2 eexists; repeat split; eauto. lia.
+        apply in_list_assoc_set_inv in H. destruct H; eauto. inv H.
+        inv H0. eapply GUARDVALID in H5. eapply var_lt_gen_r. 2: eauto. lia.
+        inv H5.
+        do 2 eexists; repeat split; eauto. lia.
+        apply in_list_assoc_set_inv in H. destruct H; eauto. inv H.
+        inv H0.
+      }
+      eapply wf_rir_incr; eauto. lia.
+      {
+        red; intros. inv H.
+        do 2 eexists; repeat split; eauto. lia.
+      }
+      specialize (H1 _ _ _ _ _ _ _ _ _ _ _ Heqp9).
+      destruct H1 as (VVSGROWS3 & VVSRANGE3 & ENVVVS3 & EXTCALL3 & VAR3 & RIRRNG3 & VVSVALID3 & VF3 & NIDGROWS3); auto.
+      {
+        intros.
+        apply ENVVVS1 in H.
+        rewrite in_map_iff in H. destruct H as ((s&a)&EQ & IN). simpl in EQ. subst.
+        replace y with (fst (y, a)). eapply in_map. apply VVSGROWS2.
+        rewrite list_assoc_set_not_before.
+        rewrite list_assoc_set_not_before.
+        rewrite list_assoc_set_not_before. auto.
+        intro IN2; eapply vvs_range_in_fst in IN2; eauto. lia.
+        intro IN2. apply in_map_list_assoc_set_inv in IN2.
+        destruct IN2. apply generate_binding_name_inj in H. lia.
+        eapply vvs_range_in_fst in H; eauto. lia.
+        intro IN2. apply in_map_list_assoc_set_inv in IN2.
+        destruct IN2. apply generate_binding_name_inj in H. lia.
+        apply in_map_list_assoc_set_inv in H.
+        destruct H. apply generate_binding_name_inj in H. lia.
+        eapply vvs_range_in_fst in H; eauto. lia.
+        reflexivity.
+      }
+      {
+        red; intros.
+        inv H.
+        do 2 eexists; repeat split; eauto. lia.
+      }
+      edestruct merge_banches_grows as (VVSGROWS4 & VVSRANGE4 & ENVVVS4 & NIDGROWS4 & VVSVALID4); eauto.
+      {
+        intros x y INl2.
+        apply ENVVVS2 in INl2.
+        rewrite in_map_iff in INl2. destruct INl2 as (xx & EQ & IN). subst. destruct xx.
+        apply VVSGROWS3 in IN. apply in_map. auto.
+      }
+      {
+        eexists; split; eauto. lia.
+      }
+      repeat (refine (conj _ _)); eauto.
+      {
+        intros. eapply VVSGROWS1 in H.
+        eapply VVSGROWS4.
+        eapply VVSGROWS3.
+        eapply VVSGROWS2.
+        rewrite ! list_assoc_set_not_before. auto.
+        intro IN2; eapply vvs_range_in_fst in IN2; eauto. lia.
+        intro IN2. apply in_map_list_assoc_set_inv in IN2.
+        destruct IN2. apply generate_binding_name_inj in H0. lia.
+        eapply vvs_range_in_fst in H0; eauto. lia.
+        intro IN2. apply in_map_list_assoc_set_inv in IN2.
+        destruct IN2. apply generate_binding_name_inj in H0. lia.
+        apply in_map_list_assoc_set_inv in H0.
+        destruct H0. apply generate_binding_name_inj in H0. lia.
+        eapply vvs_range_in_fst in H0; eauto. lia.
+      }
+      easy.
+      eapply wf_rir_incr; eauto.
+      red; intros. inv H.
+      lia.
+    - repeat (refine (conj _ _)); eauto. intros. inv H. inv H0.
+      eapply wf_rir_add_read0; eauto.
+      red; intros; inv H.
+    - repeat (refine (conj _ _)); eauto. intros. inv H. inv H0.
+      eapply wf_rir_add_read1; eauto. red; intros; inv H.
+    - specialize (H _ _ _ _ _ _ _ _ _ _ _ Heqp H2 ENVVVS RNGVVS).
+      destruct H as (VVSGROWS1 & VVSRANGE1 & ENVVVS1 & EXTCALL1 & VAR1 & RIRRNG1 & VVSVALID1 & VF1 & NIDGROWS1 ); eauto.
+      assert (valid_vars_uact guard nid'). eapply valid_var_uact_incr; eauto.
+      assert (valid_vars_uact (reduce o) nid').
+      destruct o; simpl.
+      red; intros. eapply VAR1 in H0. eapply vss_or_extcall_var_lt in H0; eauto. auto.
+      red; intros; inv H0.
+      assert (wf_rir rir' nid' /\ valid_vars_uact u0 nid').
+      {
+        destr_in Heqp4; [eapply wf_rir_add_write0 in Heqp4 | eapply wf_rir_add_write1 in Heqp4]; eauto.
+      }
+      destruct H1.
+      repeat (refine (conj _ _)); eauto. 2: easy.
+      unfold add_write0, add_write1 in Heqp4;
+        repeat destr_in Heqp4; inv Heqp4; simpl; eauto.
+      apply valid_vars_merge_failures; auto.
+
+    - specialize (H _ _ _ _ _ _ _ _ _ _ _ Heqp H2 ENVVVS RNGVVS).
+      destruct H as (VVSGROWS1 & VVSRANGE1 & ENVVVS1 & EXTCALL1 & VAR1 & RIRRNG1 & VVSVALID1 & VF1 & NIDGROWS1); eauto.
+      repeat (refine (conj _ _)); eauto. intros. inv H. inv H0.
+      destruct o. 2: inv H4. simpl in H4.
+      eapply VAR1 in H4; eauto.
+    - specialize (H _ _ _ _ _ _ _ _ _ _ _ Heqp H4 ENVVVS RNGVVS).
+      destruct H as (VVSGROWS1 & VVSRANGE1 & ENVVVS1 & EXTCALL1 & VAR1 & RIRRNG1 & VVSVALID1 & VF1 & NIDGROWS1); eauto.
+      generalize (get_rule_information_aux_same_vm _ _ _ _ _ _ _ _ _ _ _ _ H4 Heqp). intro SVM1.
+      erewrite same_env_same_fst in H6; eauto.
+      specialize (H0 _ _ _ _ _ _ _ _ _ _ _ Heqp4 H6).
+      destruct H0 as (VVSGROWS2 & VVSRANGE2 & ENVVVS2 & EXTCALL2 & VAR2 & RIRRNG2 & VVSVALID2 & VF2 & NIDGROWS2); eauto.
+      {
+        intros v VARINGUARD. apply GUARDVALID in VARINGUARD.
+        eapply var_lt_gen_r. 2: eauto. lia.
+      }
+      repeat (refine (conj _ _)); eauto.
+      intros. inv H. inv H0.
+      destruct o. 2: inv H5. simpl in H5.
+      eapply VAR1 in H5; eauto. destruct H5. left.
+      eapply incl_incl_map; eauto. decompose [ex and] H; right; eexists; split; eauto.
+      destruct o0. 2: inv H5. simpl in H5.
+      eapply VAR2 in H5; eauto.
+      apply valid_vars_merge_failures; auto. eapply valid_var_uact_incr; eauto. lia.
+    - specialize (H _ _ _ _ _ _ _ _ _ _ _ Heqp H2 ENVVVS RNGVVS).
+      destruct H as (VVSGROWS1 & VVSRANGE1 & ENVVVS1 & EXTCALL1 & VAR1 & RIRRNG1 & VVSVALID1 & VF1 & NIDGROWS1); eauto.
+      repeat refine (conj _ _); eauto.
+      eapply vvs_range_incr. 2: eauto. lia.
+      unfold add_extcall. simpl. eauto.
+      intros. inv H. inv H0. right.
+      unfold add_extcall; eexists; split; eauto.
+      simpl. left; reflexivity. reflexivity.
+
+      Lemma wf_rir_add_extcall:
+        forall rir guard ufn arg n,
+          wf_rir rir n ->
+          valid_vars_uact guard n ->
+          valid_vars_uact arg n ->
+          wf_rir (add_extcall rir guard ufn arg (generate_binding_name n)) (S n).
+      Proof.
+        intros rir guard ufn arg n WR VG VA.
+        unfold add_extcall; simpl.
+        inv WR; split; simpl; eauto using valid_var_uact_incr, wf_write_log_raw_incr.
+        intros i ext [EQ|IN]; eauto using wf_extcall_info_incr.
+        inv EQ. constructor; simpl; eauto using valid_var_uact_incr.
+        do 2 eexists; repeat split; eauto.
+      Qed.
+      eapply wf_rir_add_extcall; eauto using wf_rir_incr.
+      eapply valid_var_uact_incr; eauto.
+      destruct o; simpl.
+      red; intros. eapply VAR1 in H. eapply vss_or_extcall_var_lt in H; eauto. auto.
+      red; intros; inv H.
+      eapply valid_var_uact_incr; eauto.
+    -  
+      eapply gria_list_grows with
+        (I:= fun env vvs nid rir guard =>
+               (forall x y : string, In (x, y) env -> In y (map fst vvs))
+               /\ vvs_range vvs nid
+               /\ (forall x y, In (x, y) vvs -> forall v, var_in_uact y v -> var_lt v x)
+               /\ wf_rir rir nid
+               /\ valid_vars_uact guard nid
+        )
+        (P:= fun env vvs nid rir env' vvs' nid' rir' =>
+               Forall2 (fun x y => fst x = fst y) env env'
+               /\ (forall (x : string) (y : uact), In (x, y) vvs -> In (x, y) vvs')
+               /\ (forall ext, In ext (rir_extcalls rir) -> In ext (rir_extcalls rir'))
+               (* /\ nid <= nid' *)
+         ) in Heqp.
+      7: {
+        eapply Forall_impl.
+        2: apply H0. simpl; intros. decompose [and] H8. clear H8.
+        generalize (get_rule_information_aux_same_vm _ _ _ _ _ _ _ _ _ _ _ _ H4 H2). intro SVM1.
+        eapply H1 in H2; eauto. intuition eauto.
+        - eapply valid_var_uact_incr; eauto.
+        - red; intros.
+          eapply H16 in H22; eauto.
+          eapply var_lt_gen_r. 2: eapply vss_or_extcall_var_lt in H22; eauto. lia.
+        - eapply valid_var_uact_incr; eauto.
+      }
+      destruct Heqp as ((SAMEENV1 & (VVSGROWS1 & EXTGROWS1)) & ((ENVVVS1 & VVSRANGE1 & VVSVALID1 & RIRRNG1 & GUARDVALID1) & (NAMES & LENNAMES & VF1 & NID1))).
+      2: {
+        simpl. split. apply same_env_refl. auto.
+      }
+      2: {
+        simpl; intros; eauto.
+        decompose [and] H1; clear H1.
+        decompose [and] H2; clear H2.
+        decompose [and] H4; clear H4.
+        decompose [and] H7; clear H7.
+        repeat split; eauto.
+        eapply same_env_trans; eauto. congruence.
+      }
+      2: {
+        intros. destruct H1.
+        erewrite <- same_env_same_fst; eauto.
+      }
+      2: {
+        intuition.
+        - apply same_env_refl.
+        - rewrite list_assoc_set_not_before. auto.
+          intro IN2; eapply vvs_range_in_fst in IN2; eauto. lia.
+        - apply list_assoc_set_key_stays_in. eauto.
+        - eapply vvs_range_list_assoc_set. eapply vvs_range_incr. 2: eauto. lia.
+          eexists; split; eauto.
+        - apply in_list_assoc_set_inv in H9; destruct H9 as [EQ|IN].
+          inv EQ. eapply var_lt_gen_r. 2: eauto. lia. eauto.
+        - eapply wf_rir_incr; eauto.
+        - eapply valid_var_uact_incr; eauto.
+      }
+      2:{
+        simpl; intros. intuition; eauto.
+        rewrite in_map_iff in H4. decompose [ex and] H4. clear H4; subst. destruct x0.
+        apply in_map. eauto.
+      }
+      2: now auto.
+      2: now (eapply valid_var_uact_incr; eauto).
+      2: red; now inversion 1.
+      2: now split; auto.
+      2: constructor.
+
+      clear H0.
+      simpl in LENNAMES.
+      specialize (H _ _ _ _ _ _ _ _ _ _ _ Heqp4).
+      rewrite map_fst_combine in H.
+      rewrite fst_split_map in H. 
+      destruct H as (VVSGROWS2 & VVSRANGE2 & ENVVVS2 & EXTGROWS2 & VAR2 & RIR2 & VVSVALID2 & FV2 & NID2); auto.
+      intros x y IN; apply in_combine_r in IN.
+      rewrite Forall_forall in NAMES; apply NAMES in IN. auto.
+      repeat refine(conj _ _); eauto.
+      + intros x y IN; apply ENVVVS1 in IN.
+        rewrite in_map_iff in IN. decompose [ex and] IN. clear IN; subst. destruct x0.
+        apply in_map. eauto.
+      + eapply valid_vars_merge_failures; eauto using valid_var_uact_incr.
+      + lia.
+      + rewrite fst_split_map. setoid_rewrite H5. congruence.
+  Qed.
+
+  (* Fixpoint read_from_rirs *)
+  (*          (REnv: Env reg_t) *)
+  (*          (r: env_t REnv (fun _ => val)) *)
+  (*          (rir: rule_information_raw) *)
+  (*          (prt: Port) (idx: reg_t) : val := *)
+  (*   match prt with *)
+  (*   | P0 => getenv REnv r idx *)
+  (*   | P1 => *)
+  (*       match list_assoc (rir_writes0s rir) idx with *)
+  (*         None => getenv REnv r idx *)
+  (*       | Some (_, wil) => *)
+
+  (*       end *)
+  (*   end *)
+  (* . *)
+
+  (* Fixpoint interp_uact_with_fake_vars *)
+  (*          (u: uact) *)
+  (*          (vvs: list (string * uact)) *)
+  (*          (REnv: Env reg_t) *)
+  (*          (r: env_t REnv (fun _ => val)) *)
+  (*          (rirs: list rule_information_raw) *)
+  (*   : option val := *)
+  (*   match u with *)
+  (*   | DVar var => None          (* TODO *) *)
+  (*   | DRead port idx => *)
+  (*       None *)
+  (*   | DConst cst => Some (BitsToLists.val_of_value cst) *)
+  (*   | DIf cond tbranch fbranch => *)
+  (*       let/opt c := interp_uact_with_fake_vars cond vvs in *)
+  (*       match c with *)
+  (*       | Bits _ [true] => interp_uact_with_fake_vars tbranch vvs *)
+  (*       | Bits _ [false] => interp_uact_with_fake_vars tbranch vvs *)
+  (*       | _ => None *)
+  (*       end *)
+  (*   | DUnop ufn1 arg1 => *)
+  (*       let/opt v := interp_uact_with_fake_vars arg1 vvs in *)
+  (*       UntypedSemantics.sigma1 ufn1 v *)
+  (*   | DBinop ufn2 arg1 arg2 => *)
+  (*       let/opt v1 := interp_uact_with_fake_vars arg1 vvs in *)
+  (*       let/opt v2 := interp_uact_with_fake_vars arg2 vvs in *)
+  (*       UntypedSemantics.sigma2 ufn2 v1 v2 *)
+  (*   | DError _ *)
+  (*   | DFail _ *)
+  (*   | DAssign _ _ *)
+  (*   | DSeq _ _ *)
+  (*   | DBind _ _ _ *)
+  (*   | DWrite _ _ _ *)
+  (*   | DExternalCall _ _ *)
+  (*   | DInternalCall _ _ *)
+  (*   | DAPos _ _ => None *)
+  (*   end. *)
+
+
+  (* Lemma get_rule_information_aux_act: *)
+  (*   forall *)
+  (*     (R: reg_t -> type) *)
+  (*     (Sigma: ext_fn_t -> ExternalSignature) *)
+  (*     (ua: uact) (env: list (string * string)) (guard: uact) *)
+  (*     (rir: rule_information_raw) (nid: next_ids) *)
+  (*     v env' vvs fail_cond rir' nid' *)
+  (*     sig t *)
+  (*     (GRIA: get_rule_information_aux ua env guard rir nid = (v, env', vvs, fail_cond, rir', nid')) *)
+  (*     (TA: forall p, exists tcr, *)
+  (*         TypeInference.tc_action R Sigma p sig t ua = Success tcr) *)
+  (*     Gamma sched_log action_log action_log' v' Gamma' *)
+  (*     (REnv: Env reg_t) *)
+  (*     (r: env_t REnv (fun _ => val)) *)
+  (*     (sigma: ext_fn_t -> val -> val) *)
+  (*     (IA: UntypedSemantics.interp_action *)
+  (*            r sigma Gamma *)
+  (*            sched_log action_log ua = Some (action_log', v', Gamma')), *)
+  (*     interp_uact_with_fake_vars v vvs = Some v'. *)
+
+
+
+      
+
+  Record rule_information_raw_ok (r: rule_information_raw) (ua: uact) :=
+    {
+      rir_read0s_ok:
+      forall reg ua', In (reg, ua') (rir_read0s r) ->
+                     False;
+     
+      (* ... *)
+    }.
+
+
+  Lemma get_rule_information_raw_aux:
+    forall
+      (ua: uact) (env: list (string * string)) (guard: uact)
+      (rir: rule_information_raw) (nid: nat)
+      v env' vvs0 vvs fail_cond rir' nid',
+      get_rule_information_aux ua env vvs0 guard rir nid = (Some v, env', vvs, fail_cond, rir', nid') ->
+      rule_information_raw_ok rir ua ->
+      rule_information_raw_ok rir' ua.
+
+  Definition get_rule_information (ua: uact) (nid: nat)
+  : rule_information_raw * nat :=
     let '(_, _, vvm, failure, rule_information_raw, nid') :=
       get_rule_information_aux
-        ua [] const_true
+        ua [] [] const_true
         {| rir_read0s := []; rir_read1s := []; rir_write0s := [];
            rir_write1s := []; rir_extcalls := []; rir_vars := [];
            rir_failure_cond := None |}
         nid
     in (
-      rule_information_raw <| rir_failure_cond := failure |>
+      rule_information_raw <| rir_failure_cond := Some failure |>
         <| rir_vars := vvm|>,
       nid').
+
+  Lemma get_rule_information_ok:
+    forall ua ni r ni',
+      get_rule_information ua ni = (r, ni') ->
+      rule_information_raw_ok r ua.
+  Proof.
+  Admitted.
 
   (* * Scheduling conflicts detection *)
   (* It is here that we take into account how a rule might cancel any later
      rule. *)
   (* ** Conflicts between two rules *)
-  (* rl_failure_cond rir is used in detect_conflicts only so as to keep things
+  (* rir_failure_cond rir is used in detect_conflicts only so as to keep things
      nicely factored. *)
   Definition detect_conflicts_step
     (acc: option uact) (rir: rule_information_raw) (cond: uact) (reg: reg_t)
     (reg_failure_detection:
       rule_information_raw -> uact -> reg_t -> option uact)
-  : option uact :=
+    : option uact :=
+    (* reg_failure_detection rir cond reg && acc *)
     match reg_failure_detection rir cond reg with
     | None => acc
     | Some x =>
       match acc with
       | None => Some x
-      | Some y => Some (UBinop (PrimUntyped.UBits2 PrimUntyped.UAnd) x y)
+      | Some y => Some (uand x y)
       end
     end.
 
@@ -476,13 +2018,13 @@ Section SimpleForm.
      detect_conflicts_step. *)
   Definition detect_conflicts_read0s_reg
     (rir: rule_information_raw) (cond: uact) (reg: reg_t)
-  : option uact :=
+  : uact :=
     let prev_wr0 := option_map fst (list_assoc (rir_write0s rir) reg) in
     let prev_wr1 := option_map fst (list_assoc (rir_write1s rir) reg) in
     merge_failures_list cond (list_options_to_list [prev_wr0; prev_wr1]).
   Definition detect_conflicts_write0s_reg
     (rir: rule_information_raw) (cond: uact) (reg: reg_t)
-  : option uact :=
+  : uact :=
     let prev_wr0 := option_map fst (list_assoc (rir_write0s rir) reg) in
     let prev_rd1 := list_assoc (rir_read1s rir) reg in
     let prev_wr1 := option_map fst (list_assoc (rir_write1s rir) reg) in
@@ -490,12 +2032,12 @@ Section SimpleForm.
       cond (list_options_to_list [prev_wr0; prev_wr1; prev_rd1]).
   Definition detect_conflicts_read1s_reg
     (rir: rule_information_raw) (cond: uact) (reg: reg_t)
-  : option uact :=
+  : uact :=
     let prev_wr1 := option_map fst (list_assoc (rir_write1s rir) reg) in
     merge_failures_list cond (list_options_to_list [prev_wr1]).
   Definition detect_conflicts_write1s_reg
     (rir: rule_information_raw) (cond: uact) (reg: reg_t)
-  : option uact :=
+  : uact :=
     let prev_wr1 := option_map fst (list_assoc (rir_write1s rir) reg) in
     merge_failures_list cond (list_options_to_list [prev_wr1]).
 
@@ -513,8 +2055,8 @@ Section SimpleForm.
     (rir: rule_information_raw) (wl: write_log_raw)
   : option uact :=
     fold_left
-      (fun acc '(reg, w) =>
-        detect_conflicts_step acc rir (fst w) reg detect_conflicts_write0s_reg)
+      (fun acc '(reg, (ua,lwi)) =>
+        detect_conflicts_step acc rir ua reg detect_conflicts_write0s_reg)
       wl None.
   Definition detect_conflicts_read1s (rir: rule_information_raw) (rl: cond_log)
   : option uact :=
@@ -526,8 +2068,8 @@ Section SimpleForm.
     (rir: rule_information_raw) (wl: write_log_raw)
   : option uact :=
     fold_left
-      (fun acc '(reg, w) =>
-        detect_conflicts_step acc rir (fst w) reg detect_conflicts_write1s_reg)
+      (fun acc '(reg, (ua, lwi)) =>
+        detect_conflicts_step acc rir ua reg detect_conflicts_write1s_reg)
       wl None.
 
   (* The order of the arguments matters! If there is a conflict between a1 and
@@ -557,7 +2099,7 @@ Section SimpleForm.
          | Some y =>
            let not_failure_1 := UUnop (PrimUntyped.UBits1 PrimUntyped.UNot) y in
            (* If rule 1 fails, then it can't cause rule 2 to fail. *)
-           Some (UBinop (PrimUntyped.UBits2 PrimUntyped.UAnd) not_failure_1 x)
+           Some (DBinop (PrimUntyped.UBits2 PrimUntyped.UAnd) not_failure_1 x)
          end
        end).
 
@@ -569,6 +2111,31 @@ Section SimpleForm.
       (fun r' p => r' <| rir_failure_cond := detect_conflicts p r' |>)
       prior_rules r.
 
+
+  Definition clean_rule_information (r: rule_information_raw) :
+      rule_information_clean :=
+    {|
+      ric_write0s := map (fun '(a, (_, b)) => (a, b)) (rir_write0s r);
+      ric_write1s := map (fun '(a, (_, b)) => (a, b)) (rir_write1s r);
+      ric_extcalls := rir_extcalls r;
+      ric_vars := rir_vars r;
+      ric_failure_cond := rir_failure_cond r
+    |}.
+
+
+  Record rule_information_clean_ok (r: rule_information_clean) (ua: uact) :=
+    {
+      (* ... *)
+    }.
+
+  Lemma clean_rule_information_ok:
+    forall ua r,
+      rule_information_raw_ok r ua ->
+      rule_information_clean_ok (clean_rule_information r) ua.
+  Proof.
+  Admitted.
+
+
   (* ** All scheduling conflicts *)
   (* This function detects all the scheduling conflicts. It returns a list of
      rule_information where the failure conditions have been edited
@@ -576,20 +2143,11 @@ Section SimpleForm.
   Definition detect_all_conflicts (rl: list rule_information_raw)
   : list rule_information_clean :=
     let raw := fold_left
-      (fun acc c =>
-        match acc with
-        | [] => [c]
-        | h::t => app acc [detect_conflicts_any_prior c acc]
-        end)
+      (fun acc c => acc ++ [detect_conflicts_any_prior c acc])
       rl []
     in
-    map (fun r => {|
-      ric_write0s := map (fun '(a, (_, b)) => (a, b)) (rir_write0s r);
-      ric_write1s := map (fun '(a, (_, b)) => (a, b)) (rir_write1s r);
-      ric_extcalls := rir_extcalls r;
-      ric_vars := rir_vars r;
-      ric_failure_cond := rir_failure_cond r
-   |}) raw.
+    (* TODO: PROVE STUFF HERE *)
+    map clean_rule_information raw.
 
   (* * Schedule merger *)
   (* Starting from a schedule with all the right failures conditions under the
@@ -612,7 +2170,7 @@ Section SimpleForm.
     map
       (fun '(ufn, ei) =>
         (ufn, {|
-          econd := UBinop (PrimUntyped.UBits2 PrimUntyped.UAnd) cond (econd ei);
+          econd := DBinop (PrimUntyped.UBits2 PrimUntyped.UAnd) cond (econd ei);
           ebind := ebind ei; earg := earg ei |}))
       el.
 
@@ -719,7 +2277,7 @@ Section SimpleForm.
       app_uniq
         (find_all_ua_regs cond)
         (app_uniq (find_all_ua_regs tb) (find_all_ua_regs fb))
-    | UBinop ufn a1 a2 => app_uniq (find_all_ua_regs a1) (find_all_ua_regs a2)
+    | DBinop ufn a1 a2 => app_uniq (find_all_ua_regs a1) (find_all_ua_regs a2)
     | UUnop ufn a => find_all_ua_regs a
     | _ => []
     end.
@@ -763,8 +2321,8 @@ Section SimpleForm.
         (replace_rd1_with_var_in_uact from to cond)
         (replace_rd1_with_var_in_uact from to tb)
         (replace_rd1_with_var_in_uact from to fb)
-    | UBinop ufn a1 a2 =>
-      UBinop
+    | DBinop ufn a1 a2 =>
+      DBinop
         ufn
         (replace_rd1_with_var_in_uact from to a1)
         (replace_rd1_with_var_in_uact from to a2)
@@ -885,11 +2443,9 @@ Section SimpleForm.
     (* Get rule_information from each rule *)
     let '(rule_info_l, nid') :=
       fold_left
-        (fun '(ri_acc, nid') r =>
+        (fun '(rir_acc, nid') r =>
           let '(ri, nid'') := get_rule_information r nid' in
-          (* Not a fold right since we want the first rule to have the lowest
-             indices. *)
-          (ri_acc++[ri], nid''))
+          (rir_acc++[ri], nid''))
         rules_l ([], initial_ids)
     in
     (* Detect inter-rules conflicts *)
